Obc -> Clight proof reworked entirely! much better now I think Finally renaming RMemory into Memory seems to not be a good idea, coqdep still (apparently) undeterministically clashes with the Memory of Compcert VelusCorrectness needs to be adapted

src/ObcToClight/Correctness.v
@@ -10,11 +10,12 @@ From compcert Require Import common.Values.
 From compcert Require Import common.Memory.
 From compcert Require Import common.Events.
 From compcert Require Import common.Globalenvs.
+From compcert Require Import common.Smallstep.
 From compcert Require Import common.Behaviors.
 
 From Velus Require Import Common.
 From Velus Require Import Environment.
-From Velus Require Import Memory.
+From Velus Require Import VelusMemory.
 From Velus Require Import Ident.
 From Velus Require Import Traces.
 
@@ -164,7 +165,7 @@ Definition call_spec (prog: program) (ge: genv) (c: class) (f: method) (vs rvs: 
                m |= staterep gcenv prog c.(c_name) me sb (Ptrofs.unsigned sofs) ** P ->
                exists m' fd,
                  method_spec c f prog fd
-                 /\ eval_funcall ge (function_entry2 ge) m (Internal fd)
+                 /\ eval_funcall_fe function_entry2 ge m (Internal fd)
                                 (Vptr sb sofs :: vs) E0 m' Vundef
                  /\ m' |= staterep gcenv prog c.(c_name) me' sb (Ptrofs.unsigned sofs) ** P
              )
@@ -172,7 +173,7 @@ Definition call_spec (prog: program) (ge: genv) (c: class) (f: method) (vs rvs: 
                 m |= staterep gcenv prog c.(c_name) me sb (Ptrofs.unsigned sofs) ** P ->
                 exists m' fd rv,
                   method_spec c f prog fd
-                  /\ eval_funcall ge (function_entry2 ge) m (Internal fd)
+                  /\ eval_funcall_fe function_entry2 ge m (Internal fd)
                                  (Vptr sb sofs :: vs) E0 m' rv
                   /\ rvs = [rv]
                   /\ m' |= staterep gcenv prog c.(c_name) me' sb (Ptrofs.unsigned sofs) ** P
@@ -185,7 +186,7 @@ Definition call_spec (prog: program) (ge: genv) (c: class) (f: method) (vs rvs: 
                        ** P ->
                   exists ve_f m' fd,
                     method_spec c f prog fd
-                    /\ eval_funcall ge (function_entry2 ge) m (Internal fd)
+                    /\ eval_funcall_fe function_entry2 ge m (Internal fd)
                                    (Vptr sb sofs :: var_ptr instb :: vs) E0 m' Vundef
                     /\ Forall2 (fun xt v => Env.find (fst xt) ve_f = Some v) outs rvs
                     /\ m' |= staterep gcenv prog c.(c_name) me' sb (Ptrofs.unsigned sofs)
@@ -466,7 +467,7 @@ Section PRESERVATION.
             * now rewrite Eq.
           + destruct Struct.
             split; try omega.
-            apply (Z.le_le_add_le 0 (sizeof_struct (globalenv tprog) 0 (make_members c))); try omega.
+            apply (Z.le_le_add_le 0 (sizeof_struct (Clight.globalenv tprog) 0 (make_members c))); try omega.
             apply sizeof_struct_incr.
         Qed.
 
@@ -553,7 +554,7 @@ Section PRESERVATION.
                 ** P1 ->
           eval_expr tge e le1 m1 ae v ->
           exists m' le',
-            exec_stmt tge (function_entry2 tge) e le1 m1
+            exec_stmt_fe function_entry2 tge e le1 m1
                       (assign owner caller x (cltype ty) ae)
                       E0 le' m' Out_normal
             /\ m' |= match_out gcenv owner caller (Env.add x v ve1) le' outb_co
@@ -578,7 +579,7 @@ Section PRESERVATION.
 
           (* only one output: x is a temporary *)
           + inversion_clear Hin' as [Eq|Eq]; inv Eq.
-            exists m1, (PTree.set x v le1); rewrite PTree.gso; intuition; eauto using exec_stmt.
+            exists m1, (PTree.set x v le1); rewrite PTree.gso; intuition; unfold exec_stmt_fe; eauto using exec_stmt.
             eapply sep_imp; eauto.
             * eapply match_out_assign_singleton_mem; eauto.
             * rewrite varsrep_add; eauto.
@@ -602,7 +603,8 @@ Section PRESERVATION.
               (apply NotIn_NotInMembers; intro; apply mem_assoc_ident_false; auto).
           exists m1, (PTree.set x v le1); rewrite PTree.gso; intuition; auto.
           + unfold assign.
-            destruct_list caller.(m_out) : Houts; try rewrite E; eauto using exec_stmt.
+            destruct_list caller.(m_out) : Houts; try rewrite E;
+              unfold exec_stmt_fe; eauto using exec_stmt.
           + eapply sep_imp; eauto.
             * eapply match_out_assign_var_mem; eauto using output_match.
             * rewrite varsrep_add; eauto.
@@ -611,7 +613,7 @@ Section PRESERVATION.
       Corollary exec_assign_match_states:
           eval_expr tge e le m ae v ->
           exists m' le',
-            exec_stmt tge (function_entry2 tge) e le m
+            exec_stmt_fe function_entry2 tge e le m
                       (assign owner caller x (cltype ty) ae)
                       E0 le' m' Out_normal
             /\ m' |= match_states gcenv prog owner caller (me, Env.add x v ve) (e, le') sb sofs outb_co
@@ -707,7 +709,7 @@ Section PRESERVATION.
           wt_vals vs outs ->
           Forall2 (fun xt v => Env.find (fst xt) ve_callee = Some v) outs vs ->
           exists m' le',
-            exec_stmt tge (function_entry2 tge) e le m1
+            exec_stmt_fe function_entry2 tge e le m1
                       (funcall_assign owner caller xs o tyo outs)
                       E0 le' m' Out_normal
             /\ m' |= blockrep gcenv ve_callee (co_members instco) instb
@@ -721,7 +723,7 @@ Section PRESERVATION.
         induction outs as [|(x, t)]; intros * Hmem ??? Incl Hins WTvs Hvs;
           inversion_clear Hins as [|y]; inv WTvs; inv Hvs; unfold funcall_assign; simpl.
         - rewrite Env.adds_nil_l.
-          exists m1, le; intuition; eauto using exec_stmt.
+          exists m1, le; intuition; unfold exec_stmt_fe;  eauto using exec_stmt.
         - apply incl_cons' in Incl as (?&?).
           rewrite sep_swap, sep_swap23 in Hmem.
           edestruct exec_assign with (x := y) (ty := t) (ae := Efield (Evar o tyo) x (cltype t))
@@ -733,7 +735,7 @@ Section PRESERVATION.
           rewrite sep_swap23, sep_swap in Hmem_x.
           edestruct IHouts as (m' & le' & ? & ?); eauto.
           change E0 with (Eapp E0 (Eapp E0 E0)).
-          exists m', le'; intuition; eauto using exec_stmt.
+          exists m', le'; intuition; unfold exec_stmt_fe; eauto using exec_stmt.
       Qed.
 
       Corollary exec_funcall_assign:
@@ -743,7 +745,7 @@ Section PRESERVATION.
           wt_vals vs callee.(m_out) ->
           Forall2 (fun xt v => Env.find (fst xt) ve_callee = Some v) callee.(m_out) vs ->
           exists m' le',
-            exec_stmt tge (function_entry2 tge) e le m1
+            exec_stmt_fe function_entry2 tge e le m1
                       (funcall_assign owner caller xs o tyo callee.(m_out))
                       E0 le' m' Out_normal
             /\ m' |= blockrep gcenv ve_callee (co_members instco) instb
@@ -778,7 +780,7 @@ Section PRESERVATION.
         eval_exprlist tge e le m es (list_type_to_typelist (map Clight.typeof es)) vs ->
         wt_mem me_o' prog'' c ->
         exists m' le',
-          exec_stmt tge (function_entry2 tge) e le m
+          exec_stmt_fe function_entry2 tge e le m
                     (binded_funcall prog owner caller ys cid o fid es)
                     E0 le' m' Out_normal /\
           m' |= match_states gcenv prog owner caller
@@ -1038,7 +1040,7 @@ Section PRESERVATION.
         m |= match_states gcenv prog owner caller (me, ve) (e, le) sb sofs outb_co
              ** P ->
         exists m' le',
-          exec_stmt tge (function_entry2 tge) e le m
+          exec_stmt_fe function_entry2 tge e le m
                     (translate_stmt prog owner caller s)
                     E0 le' m' Out_normal
           /\ m' |= match_states gcenv prog owner caller (me', ve') (e, le') sb sofs outb_co
@@ -1066,7 +1068,7 @@ Section PRESERVATION.
                  (NoNaked    : No_Naked_Vars s)
                  (WTs        : wt_stmt prog' owner.(c_objs) owner.(c_mems) (meth_vars caller) s),
                exists m' le',
-                 exec_stmt tge (function_entry2 tge) e le m
+                 exec_stmt_fe function_entry2 tge e le m
                            (translate_stmt prog owner caller s) E0 le' m' Out_normal
                  /\ m' |= match_states gcenv prog owner caller (me', ve') (e, le') sb sofs outb_co ** P)
          /\
@@ -1158,8 +1160,7 @@ Section PRESERVATION.
       clear Hmem.
       edestruct IH2 as (m' & le' &?&?); eauto.
       change E0 with (Eapp E0 (Eapp E0 E0)).
-      exists m', le'; intuition; eauto using exec_stmt.
-
+      exists m', le'; intuition; unfold exec_stmt_fe; eauto using exec_stmt.
 
     (* if e then s1 else s2 *)
     - assert (Cop.bool_val v (Clight.typeof (translate_exp owner caller cond)) m = Some b)
@@ -1174,7 +1175,7 @@ Section PRESERVATION.
         eapply exec_Sifthenelse with (b := false); eauto using expr_correct.
 
     (* skip *)
-    - exists m, le; split; eauto using exec_stmt.
+    - exists m, le; split; eauto; constructor.
 
     (* funcall *)
     - eapply find_class_sub_same in Findcl; eauto.
@@ -1294,7 +1295,7 @@ Section PRESERVATION.
       m |= match_states gcenv prog owner caller (me, ve) (e, le) sb sofs outb_co
            ** P ->
       exists m' le',
-        exec_stmt tge (function_entry2 tge) e le m
+        exec_stmt_fe function_entry2 tge e le m
                   (translate_stmt prog owner caller s)
                   E0 le' m' Out_normal
         /\ m' |= match_states gcenv prog owner caller (me', ve') (e, le') sb sofs outb_co
@@ -1315,365 +1316,9 @@ Section PRESERVATION.
     intros; eapply mutual_correctness; eauto.
   Qed.
 
-
-  (* Lemma compat_auto_funcall_pres: *)
-  (*     forall f sb ob vs c prog' me tself tout callee_id callee instco m ob_co P, *)
-  (*       let vargs := var_ptr sb *)
-  (*                         :: match callee.(m_out) with *)
-  (*                           | [] | [_] => vs *)
-  (*                           | _ => var_ptr ob :: vs *)
-  (*                           end *)
-  (*       in *)
-  (*       find_class c.(c_name) prog = Some (c, prog') -> *)
-  (*       find_method callee_id c.(c_methods) = Some callee -> *)
-  (*       length f.(fn_params) = length vargs -> *)
-  (*       fn_params f = (self, tself) *)
-  (*                       :: match callee.(m_out) with *)
-  (*                         | [] | [_] => map translate_param callee.(m_in) *)
-  (*                         | _ => (out, tout) :: map translate_param callee.(m_in) *)
-  (*                         end -> *)
-  (*       fn_vars f = make_out_vars (instance_methods callee) -> *)
-  (*       fn_temps f = match callee.(m_out) with *)
-  (*                    | [yt] => [translate_param yt] *)
-  (*                    | _ => [] *)
-  (*                    end *)
-  (*                      ++ make_out_temps (instance_methods_temp (rev prog) callee) *)
-  (*                      ++ map translate_param callee.(m_vars) -> *)
-  (*       list_norepet (var_names f.(fn_params)) -> *)
-  (*       list_norepet (var_names f.(fn_vars)) -> *)
-  (*       match callee.(m_out) with *)
-  (*       | [] | [_] => True *)
-  (*       | _ => *)
-  (*         ob_co = Some (ob, instco) *)
-  (*         /\ gcenv ! (prefix_fun c.(c_name) callee.(m_name)) = Some instco *)
-  (*       end -> *)
-  (*       m |= staterep gcenv prog c.(c_name) me sb Z0 *)
-  (*                                           ** match callee.(m_out) with *)
-  (*                                              | [] | [_] => sepemp *)
-  (*                                              | _ => blockrep gcenv vempty instco.(co_members) ob *)
-  (*                                              end *)
-  (*                                           ** P -> *)
-  (*       exists e_fun le_fun m_fun, *)
-  (*         bind_parameter_temps f.(fn_params) vargs (create_undef_temps f.(fn_temps)) = Some le_fun *)
-  (*         /\ alloc_variables tge empty_env m f.(fn_vars) e_fun m_fun *)
-  (*         /\ (forall x b t, e_fun ! x = Some (b, t) -> exists o f, x = prefix_out o f) *)
-  (*         /\ le_fun ! self = Some (var_ptr sb) *)
-  (*         /\ m_fun |= staterep gcenv prog c.(c_name) me sb Z0 *)
-  (*                     ** match_out c callee (Env.adds (map fst callee.(m_in)) vs vempty) le_fun ob_co *)
-  (*                     ** subrep callee e_fun *)
-  (*                     ** (subrep callee e_fun -* subrep_range e_fun) *)
-  (*                     ** varsrep callee (Env.adds (map fst callee.(m_in)) vs vempty) le_fun *)
-  (*                     ** P. *)
-  (*   Proof. *)
-  (*     intros * Findc Hcallee Hlengths *)
-  (*            Hparams Hvars Htemps Norep_par Norep_vars Hinstco Hrep. *)
-  (*     subst vargs; rewrite Hparams, Hvars, Htemps in *. *)
-  (*     assert (~ InMembers self (meth_vars callee)) as Notin_s *)
-  (*         by apply m_notreserved, in_eq. *)
-  (*     assert (~ InMembers out (meth_vars callee)) as Notin_o *)
-  (*         by apply m_notreserved, in_cons, in_eq. *)
-  (*     assert (~ InMembers self (map translate_param (m_in callee))). *)
-  (*     { unfold meth_vars in Notin_s; apply NotInMembers_app in Notin_s. *)
-  (*       rewrite fst_InMembers, translate_param_fst, <-fst_InMembers; tauto. *)
-  (*     } *)
-  (*     assert (~ InMembers self (map translate_param (m_out callee))). *)
-  (*     { unfold meth_vars in Notin_s; repeat rewrite NotInMembers_app in Notin_s. *)
-  (*       rewrite fst_InMembers, translate_param_fst, <-fst_InMembers; tauto. *)
-  (*     } *)
-  (*     assert (~ InMembers out (map translate_param (m_in callee))). *)
-  (*     { unfold meth_vars in Notin_o; apply NotInMembers_app in Notin_o. *)
-  (*       rewrite fst_InMembers, translate_param_fst, <-fst_InMembers; tauto. *)
-  (*     } *)
-  (*     assert (~ InMembers self (map translate_param (m_vars callee))). *)
-  (*     { unfold meth_vars in Notin_s; rewrite Permutation_app_comm, <-app_assoc in Notin_s; *)
-  (*         apply NotInMembers_app in Notin_s. *)
-  (*       rewrite fst_InMembers, translate_param_fst, <-fst_InMembers; tauto. *)
-  (*     } *)
-  (*     assert (~ InMembers out (map translate_param (m_vars callee))). *)
-  (*     { unfold meth_vars in Notin_o; rewrite Permutation_app_comm, <-app_assoc in Notin_o; *)
-  (*         apply NotInMembers_app in Notin_o. *)
-  (*       rewrite fst_InMembers, translate_param_fst, <-fst_InMembers; tauto. *)
-  (*     } *)
-  (*     assert (~ InMembers self (make_out_temps (instance_methods_temp (rev prog) callee))). *)
-  (*     { intro Hin_s. *)
-  (*       apply make_out_temps_prefixed in Hin_s. *)
-  (*       apply self_not_prefixed; auto. *)
-  (*     } *)
-  (*     assert (~ InMembers out (make_out_temps (instance_methods_temp (rev prog) callee))). *)
-  (*     { intro Hin_o. *)
-  (*       apply make_out_temps_prefixed in Hin_o. *)
-  (*       apply out_not_prefixed; auto. *)
-  (*     } *)
-
-  (*     assert (NoDupMembers (map translate_param (m_in callee))). *)
-  (*     { pose proof (m_nodupvars callee) as Nodup. *)
-  (*       rewrite Permutation_app_comm in Nodup. *)
-  (*       apply NoDupMembers_app_r in Nodup. *)
-  (*       rewrite fst_NoDupMembers, translate_param_fst, <-fst_NoDupMembers; auto. *)
-  (*     } *)
-  (*     assert (Forall (fun xt => sizeof tge (snd xt) <= Int.max_unsigned /\ *)
-  (*                            (exists (id : AST.ident) (co : composite), *)
-  (*                                snd xt = Tstruct id noattr /\ *)
-  (*                                gcenv ! id = Some co /\ *)
-  (*                                co_su co = Struct /\ *)
-  (*                                NoDupMembers (co_members co) /\ *)
-  (*                                (forall (x' : AST.ident) (t' : Ctypes.type), *)
-  (*                                    In (x', t') (co_members co) -> *)
-  (*                                    exists chunk : AST.memory_chunk, *)
-  (*                                      access_mode t' = By_value chunk /\ *)
-  (*                                      (align_chunk chunk | alignof gcenv t')))) *)
-  (*                    (make_out_vars (instance_methods callee))) *)
-  (*       by (eapply instance_methods_caract; eauto). *)
-  (*     assert (NoDupMembers (make_out_vars (instance_methods callee))) *)
-  (*       by (unfold var_names in Norep_vars; now rewrite fst_NoDupMembers, NoDup_norepet). *)
-
-  (*     destruct_list (m_out callee) as (y, t) ? ? : E. *)
-  (*     - edestruct *)
-  (*         (bind_parameter_temps_exists_noout (map translate_param callee.(m_in)) self *)
-  (*                                            (make_out_temps (instance_methods_temp (rev prog) callee) *)
-  (*                                                            ++ map translate_param callee.(m_vars)) vs *)
-  (*                                            tself (var_ptr sb)) *)
-  (*         as (le_fun & Bind & Hinputs); eauto. *)
-  (*       + rewrite NotInMembers_app; auto. *)
-  (*       + edestruct (alloc_result callee) as (e_fun & m_fun & ? & ? & Hm_fun); eauto. *)
-  (*         assert (le_fun ! self = Some (var_ptr sb)) by *)
-  (*             (eapply (bind_parameter_temps_implies'_noout (map translate_param (m_in callee))); eauto). *)
-  (*         exists e_fun, le_fun, m_fun; *)
-  (*           split; [|split; [|split; [|split]]]; auto. *)
-  (*         rewrite sep_swap4, <-sepemp_left in Hm_fun. *)
-  (*         rewrite sep_swap, match_out_nil; auto. *)
-  (*         rewrite <- 2 sep_assoc, sep_swap. *)
-  (*         rewrite translate_param_fst in Hinputs. *)
-  (*         apply sep_pure; split; auto. *)
-  (*         * rewrite map_app; simpl in Hinputs; repeat rewrite Forall_app in Hinputs. *)
-  (*           rewrite Forall_app; tauto. *)
-  (*         * rewrite sep_assoc, sep_swap, sep_assoc; auto. *)
-
-  (*     - edestruct *)
-  (*         (bind_parameter_temps_exists_noout (map translate_param callee.(m_in)) self *)
-  (*                                            (translate_param (y, t) :: *)
-  (*                                                             make_out_temps (instance_methods_temp (rev prog) callee) *)
-  (*                                                             ++ map translate_param callee.(m_vars)) vs *)
-  (*                                            tself (var_ptr sb)) *)
-  (*         as (le_fun & Bind & Hinputs); eauto. *)
-  (*       + rewrite cons_is_app. repeat rewrite NotInMembers_app; tauto. *)
-  (*       + edestruct (alloc_result callee) as (e_fun & m_fun & ? & ? & Hm_fun); eauto. *)
-  (*         assert (le_fun ! self = Some (var_ptr sb)) by *)
-  (*             (eapply (bind_parameter_temps_implies'_noout (map translate_param (m_in callee))); eauto). *)
-  (*         simpl. *)
-  (*         exists e_fun, le_fun, m_fun; *)
-  (*           split; [|split; [|split; [|split]]]; auto. *)
-  (*         rewrite sep_swap4, <-sepemp_left in Hm_fun. *)
-  (*         rewrite sep_swap, match_out_singleton; eauto; split. *)
-  (*         *{ rewrite <- 2 sep_assoc, sep_swap. *)
-  (*            rewrite translate_param_fst in Hinputs. *)
-  (*            apply sep_pure; split; auto. *)
-  (*            - rewrite map_app; simpl in Hinputs; rewrite Forall_app, Forall_cons2, Forall_app in Hinputs. *)
-  (*              rewrite Forall_app; tauto. *)
-  (*            - rewrite sep_assoc, sep_swap, sep_assoc; auto. *)
-  (*          } *)
-  (*         *{ pose proof (m_nodupvars callee) as Nodup. *)
-  (*            rewrite Permutation_app_comm, <-app_assoc, E in Nodup. *)
-  (*            apply NoDupMembers_app_r in Nodup. *)
-  (*            rewrite <-cons_is_app in Nodup. *)
-  (*            inversion_clear Nodup as [|? ? ? Notin]. *)
-  (*            rewrite fst_InMembers in Notin. *)
-  (*            rewrite Env.gsso, Env.gempty; auto. *)
-  (*            rewrite <-fst_InMembers in Notin. *)
-  (*            eapply bind_parameter_temps_conservation; eauto. *)
-  (*            - apply NotInMembers_cons; split. *)
-  (*              + rewrite InMembers_translate_param_idem; auto. *)
-  (*              + simpl in *; auto. *)
-  (*            - simpl; apply PTree.gss. *)
-  (*          } *)
-
-  (*     - destruct Hinstco. *)
-  (*       edestruct *)
-  (*         (bind_parameter_temps_exists (map translate_param callee.(m_in)) self out *)
-  (*                                      (make_out_temps (instance_methods_temp (rev prog) callee) *)
-  (*                                                      ++ map translate_param callee.(m_vars)) vs *)
-  (*                                      tself tout (var_ptr sb) (var_ptr ob)) *)
-  (*         with (1:=self_not_out) as (le_fun & Bind & Hinputs); eauto. *)
-  (*       + rewrite NotInMembers_app; auto. *)
-  (*       + rewrite NotInMembers_app; auto. *)
-  (*       + simpl in Hlengths. inversion Hlengths; eauto. *)
-  (*       + edestruct (alloc_result callee) as (e_fun & m_fun & ? & ? & Hm_fun); eauto. *)
-  (*         edestruct (bind_parameter_temps_implies' (map translate_param (m_in callee))) *)
-  (*           with (1:=self_not_out) as (? & ?); eauto. *)
-  (*         exists e_fun, le_fun, m_fun; *)
-  (*           split; [|split; [|split; [|split]]]; auto. *)
-  (*         assert (1 < length callee.(m_out))%nat by (rewrite E; simpl; omega). *)
-  (*         rewrite sep_swap, match_out_notnil; auto; *)
-  (*           do 2 econstructor; split; [|split]; eauto. *)
-  (*         rewrite sep_swap, <- 3 sep_assoc, sep_swap. *)
-  (*         rewrite translate_param_fst in Hinputs. *)
-  (*         apply sep_pure; split; auto. *)
-  (*         * rewrite map_app; simpl in Hinputs; repeat rewrite Forall_app in Hinputs. *)
-  (*           rewrite Forall_app; tauto. *)
-  (*         * rewrite sep_assoc, sep_swap, sep_assoc, sep_swap23, sep_swap. *)
-  (*           eapply sep_imp; eauto. *)
-  (*           apply sep_imp'; auto. *)
-  (*           rewrite sep_assoc. *)
-  (*           apply sep_imp'; auto. *)
-  (*           apply sep_imp'; auto. *)
-  (*           rewrite <-translate_param_fst. *)
-  (*           erewrite <-output_match; eauto. *)
-  (*           apply blockrep_nodup. *)
-  (*           pose proof (m_nodupvars callee) as Nodup. *)
-  (*           rewrite app_assoc, Permutation_app_comm, app_assoc, Permutation_app_comm in Nodup. *)
-  (*           apply NoDupMembers_app_r in Nodup; rewrite Permutation_app_comm in Nodup. *)
-  (*           rewrite <-map_app, fst_NoDupMembers, translate_param_fst, <-fst_NoDupMembers; auto. *)
-  (*   Qed. *)
-
-  (*   Lemma corres_auto_funcall: *)
-  (*     forall me1 clsid fid vs me2 rvs c callee cf ptr_f prog' m1 sb outb outco P, *)
-  (*       let oty := type_of_inst (prefix_fun clsid fid) in *)
-  (*       stmt_call_eval prog me1 clsid fid (map Some vs) me2 (map Some rvs) -> *)
-  (*       find_class clsid prog = Some (c, prog') -> *)
-  (*       find_method fid c.(c_methods) = Some callee -> *)
-  (*       m1 |= staterep gcenv prog c.(c_name) me1 sb Z0 *)
-  (*                                            ** match callee.(m_out) with *)
-  (*                                               | [] | [_] => sepemp *)
-  (*                                               | _ => blockrep gcenv vempty outco.(co_members) outb *)
-  (*                                               end *)
-  (*                                            ** P -> *)
-  (*       wt_mem me1 prog' c -> *)
-  (*       Forall2 (fun (v : val) (xt : ident * type) => wt_val v (snd xt)) vs (m_in callee) -> *)
-  (*       Globalenvs.Genv.find_symbol tge (prefix_fun clsid fid) = Some ptr_f -> *)
-  (*       Globalenvs.Genv.find_funct_ptr tge ptr_f = Some (Ctypes.Internal cf) -> *)
-  (*       length cf.(fn_params) = (match callee.(m_out) with *)
-  (*                                | [] | [_] => 1 *)
-  (*                                | _ => 2 *)
-  (*                                end + length vs)%nat -> *)
-  (*       match callee.(m_out) with *)
-  (*       | [] | [_] => True *)
-  (*       | _ => gcenv ! (prefix_fun clsid fid) = Some outco *)
-  (*       end -> *)
-  (*       wt_stmt prog c.(c_objs) c.(c_mems) (meth_vars callee) callee.(m_body) -> *)
-  (*       exists m2, *)
-  (*         eval_funcall tge (function_entry2 tge) m1 (Internal cf) *)
-  (*                      (var_ptr sb *)
-  (*                            :: match callee.(m_out) with *)
-  (*                              | [] | [_] => vs *)
-  (*                              | _ => var_ptr outb :: vs *)
-  (*                              end) E0 m2 *)
-  (*                      match rvs with *)
-  (*                      | [v] => v *)
-  (*                      | _ => Vundef *)
-  (*                      end *)
-  (*         /\ m2 |= staterep gcenv prog c.(c_name) me2 sb Z0 *)
-  (*                                                ** match callee.(m_out) with *)
-  (*                                                   | [] | [_] => sepemp *)
-  (*                                                   | _ => blockrep gcenv (Env.adds (map fst callee.(m_out)) rvs vempty) outco.(co_members) outb *)
-  (*                                                   end *)
-  (*                                                ** P. *)
-  (*   Proof. *)
-  (*     intros ????????????????? Heval Findc Findm Hm1 Wtmem ? Hgetptrf Hgetcf ? ? ?. *)
-
-  (*     edestruct pres_sem_stmt_call with (6:=Heval) as (? & WT_val); eauto; try rewrite Forall2_map_1; auto. *)
-  (*     inversion_clear Heval as [??????????? Findc' Findm' ? Hev Hvars]. *)
-  (*     rewrite Findc' in Findc; inv Findc; *)
-  (*       rewrite Findm' in Findm; inv Findm. *)
-  (*     assert (sub_prog prog' prog) by (eapply find_class_sub; eauto). *)
-  (*     eapply stmt_eval_sub_prog in Hev; eauto. *)
-  (*     eapply wt_mem_sub in Wtmem; eauto; inv Wtmem. *)
-
-  (*     (* get the clight function *) *)
-  (*     edestruct methods_corres *)
-  (*       as (ptr_f' & cf' & Hgetptrf' & Hgetcf' & Hparams & Hret & ? & ? & ? & ? & ? & ? & Htr); eauto. *)
-  (*     rewrite Hgetptrf' in Hgetptrf; inv Hgetptrf; *)
-  (*       rewrite Hgetcf' in Hgetcf; inv Hgetcf. *)
-
-  (*     pose proof (find_class_name _ _ _ _ Findc') as Eq; *)
-  (*       pose proof (find_method_name _ _ _ Findm') as Eq'; *)
-  (*       rewrite <-Eq, <-Eq' in *. *)
-
-  (*     assert (length (fn_params cf) = *)
-  (*             length (var_ptr sb :: match m_out callee with *)
-  (*                                        | [] | [_] => vs *)
-  (*                                        | _ :: _ => var_ptr outb :: vs *)
-  (*                                        end)) *)
-  (*       by (destruct_list callee.(m_out); simpl; auto). *)
-  (*     assert (length rvs = length callee.(m_out)) *)
-  (*       by (now apply Forall2_length in Hvars; rewrite 2 map_length in Hvars). *)
-
-  (*     assert (NoDup (map fst (m_in callee))) by apply fst_NoDupMembers, m_nodupin. *)
-
-  (*     edestruct compat_auto_funcall_pres with (vs:=vs) (2:=Findm') *)
-  (*       as (e & le & m & ? & ? & ? & ? & Hm); eauto; simpl; auto. *)
-  (*     - destruct_list callee.(m_out); auto. *)
-  (*     - edestruct stmt_correctness with (p:=prog) (s:=callee.(m_body)) as (le' & m' & Hexec & MS); eauto. *)
-  (*       + apply find_class_In in Findc'; apply find_method_In in Findm'. *)
-  (*         do 2 eapply Forall_forall in NO_NAKED_VARS; eauto. *)
-  (*       + rewrite match_states_conj; split; [|split; [|repeat split; eauto]]. *)
-  (*         * rewrite Env.adds_opt_is_adds; auto. *)
-  (*           rewrite Ptrofs.unsigned_zero, sep_swap45; eauto. *)
-  (*         * rewrite Ptrofs.unsigned_zero. split; try omega. *)
-  (*           simpl. *)
-  (*           edestruct make_members_co as (co & Hco & Hsu & Hmb & ? & ? & Hbound); eauto. *)
-  (*           transitivity co.(co_sizeof); auto. *)
-  (*           erewrite co_consistent_sizeof; eauto. *)
-  (*           rewrite Hsu, Hmb. *)
-  (*           apply align_le. *)
-  (*           erewrite co_consistent_alignof; eauto. *)
-  (*           apply alignof_composite_pos. *)
-  (*         * apply wt_env_params; rewrite Forall2_map_1; auto. *)
-  (*         * rewrite Ptrofs.unsigned_zero; omega. *)
-  (*       + rewrite match_states_conj in MS; destruct MS as (Hm_fun' & ?). *)
-  (*         rewrite sep_swap23, sep_swap5, sep_swap in Hm_fun'. *)
-  (*         rewrite <-sep_assoc, sep_unwand in Hm_fun'; auto. *)
-  (*         edestruct free_exists as (m_fun'' & Hfree & Hm_fun''); eauto. *)
-  (*         exists m_fun''; split. *)
-  (*         *{ destruct_list callee.(m_out) as (?, ?)  ? ? : Out; destruct_list rvs; contr. *)
-  (*            - eapply eval_funcall_internal; eauto. *)
-  (*              + constructor; eauto. *)
-  (*              + rewrite Htr. *)
-  (*                change E0 with (Eapp E0 E0). *)
-  (*                eapply exec_Sseq_1; eauto. *)
-  (*                apply exec_Sreturn_none. *)
-  (*              + rewrite Hret; reflexivity. *)
-  (*            - eapply eval_funcall_internal; eauto. *)
-  (*              + constructor; eauto. *)
-  (*              + rewrite Htr. *)
-  (*                change E0 with (Eapp E0 E0). *)
-  (*                eapply exec_Sseq_1; eauto. *)
-  (*                apply exec_Sreturn_some. *)
-  (*                rewrite sep_swap, match_out_singleton in Hm_fun'; eauto; *)
-  (*                  destruct Hm_fun' as (Hm_fun' & Find'). *)
-  (*                inversion_clear Hvars as [|? ? ? ? Find]; rewrite Find in Find'. *)
-  (*                econstructor; eauto. *)
-  (*              + rewrite Hret; simpl; split. *)
-  (*                * destruct t; intro; contr. *)
-  (*                * inversion_clear WT_val; apply sem_cast_same; auto. *)
-  (*            - eapply eval_funcall_internal; eauto. *)
-  (*              + constructor; eauto. *)
-  (*              + rewrite Htr. *)
-  (*                change E0 with (Eapp E0 E0). *)
-  (*                eapply exec_Sseq_1; eauto. *)
-  (*                apply exec_Sreturn_none. *)
-  (*              + rewrite Hret; reflexivity. *)
-  (*          } *)
-  (*         *{ rewrite sep_swap. *)
-  (*            destruct_list (m_out callee) as (?, ?) ? ? : Out. *)
-  (*            - rewrite 2 sep_drop in Hm_fun''. *)
-  (*              rewrite <-sepemp_left; auto. *)
-  (*            - rewrite 2 sep_drop in Hm_fun''. *)
-  (*              rewrite <-sepemp_left; auto. *)
-  (*            - assert (1 < length callee.(m_out))%nat by (rewrite Out; simpl; omega). *)
-  (*              rewrite match_out_notnil in Hm_fun''; auto; destruct Hm_fun'' as (? & ? & E & Hm_fun'' & ? & ?). *)
-  (*              inversion E; subst outb outco. *)
-  (*              eapply sep_imp; eauto. *)
-  (*              + rewrite <-Out. *)
-  (*                erewrite <-output_match; eauto. *)
-  (*                rewrite <-translate_param_fst. *)
-  (*                rewrite <-Env.adds_opt_is_adds. *)
-  (*                * apply blockrep_findvars. *)
-  (*                  rewrite translate_param_fst, Out; auto. *)
-  (*                * rewrite translate_param_fst. *)
-  (*                  apply fst_NoDupMembers, m_nodupout. *)
-  (*              + rewrite sep_drop; apply sep_imp'; auto. *)
-  (*          } *)
-  (*   Qed. *)
+  (*****************************************************************)
+  (** Correctness of the whole program                            **)
+  (*****************************************************************)
 
   Let c_main     := c_main _ _ _ _ _ TRANSL.
   Let prog_main  := prog_main _ _ _ _ _ TRANSL.
@@ -1731,69 +1376,69 @@ Section PRESERVATION.
   Let out_step   := prefix out step.
   Let t_out_step := type_of_inst (prefix_fun main_node step).
 
+  (* !!!: do not use case_out or match on outputs directly because of further dependent destruction failure *)
   Lemma main_entry:
     forall m0 sb,
       m0 |= staterep gcenv prog main_node mempty sb Z0 ->
-      case_out main_step
-               (function_entry2 (globalenv tprog) main_f [] m0 empty_env le_main m0)
-               (fun _ _ => function_entry2 (globalenv tprog) main_f [] m0 empty_env le_main m0)
-               (fun _ =>
-                  exists m1 step_b step_co,
-                    function_entry2 (globalenv tprog) main_f [] m0
-                                    (PTree.set out_step (step_b, t_out_step) empty_env) le_main m1
-                    /\ gcenv ! (prefix_fun main_node step) = Some step_co
-                    /\ m1 |= staterep gcenv prog main_node mempty sb Z0
-                            ** blockrep gcenv vempty step_co.(co_members) step_b).
+      if lt_dec 1 (length (m_out main_step))
+      then
+        exists m1 step_b step_co,
+          function_entry2 tge main_f [] m0
+                          (PTree.set out_step (step_b, t_out_step) empty_env) le_main m1
+          /\ gcenv ! (prefix_fun main_node step) = Some step_co
+          /\ m1 |= staterep gcenv prog main_node mempty sb Z0
+                  ** blockrep gcenv vempty step_co.(co_members) step_b
+      else function_entry2 tge main_f [] m0 empty_env le_main m0.
   Proof.
     intros * Hmem.
     assert (list_norepet (var_names (fn_vars main_f))) by apply norepet_vars_main.
     assert (list_norepet (var_names (fn_params main_f))) by apply norepet_params_main.
     assert (list_disjoint (var_names (fn_params main_f)) (var_names (fn_temps main_f)))
       by apply disjoint_params_temps_main.
-
-    subst main_step; unfold case_out;
-      destruct_list (m_out (GenerationProperties.main_step _ _ _ _ _ TRANSL)) as (?,?) (?,?) ? : Hout.
-    - constructor; auto.
-      simpl; unfold case_out; rewrite Hout; constructor.
-    - constructor; auto.
-      simpl; unfold case_out; rewrite Hout; constructor.
-    - assert (1 < Datatypes.length (m_out (GenerationProperties.main_step _ _ _ _ _ TRANSL)))%nat
-             by (rewrite Hout; simpl; omega).
-      edestruct main_with_output_structure as (m1 & step_b & step_co &?&?& Hm1); eauto.
+    cases.
+    - edestruct main_with_output_structure as (m1 & step_b & step_co &?&?& Hm1); eauto.
       rewrite sep_comm in Hm1.
       exists m1, step_b, step_co; intuition.
       constructor; auto.
+    - constructor; auto.
+      simpl; unfold main_step, case_out in *.
+      cases; simpl in *; try omega; constructor.
   Qed.
 
   (*****************************************************************)
   (** Trace semantics of reads and writes to volatiles             *)
   (*****************************************************************)
 
-  Remark prefix_out_env_no_glob_id:
+  Definition out_step_env (e: Clight.env) : Prop :=
+    forall x b t,
+      e ! x = Some (b, t) ->
+      x = out_step.
+
+  Remark out_step_env_no_glob_id:
     forall e x,
       valid x ->
-      prefix_out_env e ->
+      out_step_env e ->
       e ! (glob_id x) = None.
   Proof.
     intros * Valid He.
     rewrite <-not_Some_is_None.
     intros (b, t') Hget.
-    apply He in Hget as (?&?& E).
+    apply He in Hget.
     apply (glob_id_not_prefixed x); auto.
-    rewrite E; constructor.
+    rewrite Hget. constructor.
   Qed.
 
   Lemma exec_read:
     forall vs e le m,
-      prefix_out_env e ->
+      out_step_env e ->
       wt_vals vs main_step.(m_in) ->
       exists le',
-        exec_stmt tge (function_entry2 tge) e le m
+        exec_stmt_fe function_entry2 tge e le m
                   (load_in main_step.(m_in))
                   (load_events vs main_step.(m_in))
                   le' m Out_normal
         /\ Forall2 (fun v xt => le' ! (fst xt) = Some v) vs main_step.(m_in)
-        /\ (forall x, ~ InMembers x main_step.(m_in) -> le' ! x = le ! x). (* TODO: needed? *)
+        /\ (forall x, ~ InMembers x main_step.(m_in) -> le' ! x = le ! x).
   Proof.
     pose proof (m_nodupin main_step) as Hnodup.
     pose proof (m_good_in main_step) as Good.
@@ -1811,7 +1456,7 @@ Section PRESERVATION.
       destruct Findx as (bx & Findx & Volx).
       rewrite load_events_cons.
       assert (exists le',
-                 exec_stmt (globalenv tprog) (function_entry2 (globalenv tprog)) e le m
+                 exec_stmt_fe function_entry2 tge e le m
                            (Sbuiltin (Some x) (AST.EF_vload (type_chunk t))
                                      (Ctypes.Tcons (Tpointer (cltype t) noattr) Ctypes.Tnil)
                                      [Eaddrof (Evar (glob_id x) (cltype t)) (Tpointer (cltype t) noattr)])
@@ -1828,7 +1473,7 @@ Section PRESERVATION.
         econstructor.
         - econstructor; eauto using eval_exprlist.
           + apply eval_Eaddrof, eval_Evar_global; eauto.
-            apply prefix_out_env_no_glob_id; auto.
+            apply out_step_env_no_glob_id; auto.
             apply (Good (x, t)), in_eq.
           + unfold Cop.sem_cast; simpl; eauto.
         - constructor.
@@ -1856,13 +1501,13 @@ Section PRESERVATION.
       (1 < Datatypes.length (m_out main_step))%nat ->
       forall rvs e ve le m step_b step_co,
         NoDupMembers outs ->
-        prefix_out_env e ->
+        out_step_env e ->
         wt_vals rvs outs ->
         gcenv ! (prefix_fun main_node step) = Some step_co ->
         e ! out_step = Some (step_b, t_out_step) ->
         Forall2 (fun xt v => Env.find (fst xt) ve = Some v) outs rvs ->
         m |= blockrep gcenv ve (co_members step_co) step_b ->
-        exec_stmt tge (function_entry2 tge) e le m
+        exec_stmt_fe function_entry2 tge e le m
                   (write_multiple_outs main_node outs)
                   (store_events rvs outs)
                   le m Out_normal.
@@ -1873,8 +1518,9 @@ Section PRESERVATION.
     assert (Forall ValidId outs) as Good
         by (apply Forall_incl with (2 := Incl), Forall_forall, m_good_out).
 
+    unfold exec_stmt_fe.
     induction outs as [|(x, t)]; intros * Nodup He WTrvs Hrco Findstr Hrvs Hm.
-    - unfold store_events; rewrite mk_event_nil; eauto using exec_stmt.
+    - rewrite store_events_nil; constructor.
     - inversion_clear Vol as [|? ? Findx];  destruct Findx as (bx & Findx & Volx).
       inversion_clear Good as [|?? Good_x].
       inversion WTrvs as [|rv ? rvs']; subst.
@@ -1894,7 +1540,7 @@ Section PRESERVATION.
           end.
         * econstructor.
           apply eval_Evar_global; eauto.
-          apply prefix_out_env_no_glob_id; auto.
+          apply out_step_env_no_glob_id; auto.
           apply Good_x.
         * reflexivity.
         * eapply sem_cast_same; eauto.
@@ -1906,7 +1552,7 @@ Section PRESERVATION.
 
   Corollary exec_write:
     forall rvs e le m,
-      prefix_out_env e ->
+      out_step_env e ->
       wt_vals rvs main_step.(m_out) ->
       case_out main_step
                True
@@ -1917,7 +1563,7 @@ Section PRESERVATION.
                     /\ e ! out_step = Some (step_b, t_out_step)
                     /\ Forall2 (fun xt v => Env.find (fst xt) ve = Some v) outs rvs
                     /\ m |= blockrep gcenv ve (co_members step_co) step_b) ->
-      exec_stmt tge (function_entry2 tge) e le m
+      exec_stmt_fe function_entry2 tge e le m
                 (write_out main_node main_step.(m_out))
                 (store_events rvs main_step.(m_out))
                 le m Out_normal.
@@ -1928,11 +1574,12 @@ Section PRESERVATION.
     assert (length rvs = length main_step.(m_out)) as Length by (eapply Forall2_length; eauto).
 
     unfold case_out in Hrep.
+    unfold exec_stmt_fe.
     destruct_list (m_out main_step) as (y, t) (y', t') outs : Out;
       destruct_list rvs as rv rv' rvs' : Rvs; contr.
 
     (* no output *)
-    - unfold store_events; rewrite mk_event_nil; eauto using exec_stmt.
+    - rewrite store_events_nil; eauto using exec_stmt.
 
     (* one output *)
     - unfold write_out.
@@ -1947,7 +1594,7 @@ Section PRESERVATION.
           end.
         * econstructor.
           apply eval_Evar_global; eauto.
-          apply prefix_out_env_no_glob_id; auto.
+          apply out_step_env_no_glob_id; auto.
           apply (Good (y, t)), in_eq.
         * reflexivity.
         * econstructor; eauto.
@@ -1966,421 +1613,6 @@ Section PRESERVATION.
       + rewrite <-Out; apply m_nodupout.
   Qed.
 
-
-  (* Section MainProgram. *)
-
-
-  (*   Let out_step   := prefix out step. *)
-  (*   Let t_out_step := type_of_inst (prefix_fun main_node step). *)
-
-  (*   (* Variables (c_main         : class) *) *)
-  (*   (*           (prog_main      : program) *) *)
-  (*   (*           (m_reset m_step : method). *) *)
-
-  (*   (* Hypothesis Find      : find_class main_node prog = Some (c_main, prog_main). *) *)
-  (*   (* Hypothesis Findreset : find_method reset c_main.(c_methods) = Some m_reset. *) *)
-  (*   (* Hypothesis Findstep  : find_method step c_main.(c_methods) = Some m_step. *) *)
-
-  (*   (* XXX: to be discharged from generation function *) *)
-  (*   Hypothesis Reset_in_spec  : main_reset.(m_in) = []. *)
-  (*   Hypothesis Reset_out_spec : main_reset.(m_out) = []. *)
-  (*   Hypothesis Step_in_spec   : main_step.(m_in) <> []. *)
-  (*   Hypothesis Step_out_spec  : main_step.(m_out) <> []. *)
-
-  (*   (* Hypothesis Step_in  : Forall is_volatile m_step.(m_in). *) *)
-  (*   (* Hypothesis Step_out : Forall is_volatile m_step.(m_out). *) *)
-
-  (*   Variables (rst_ptr stp_ptr : block) *)
-  (*             (reset_f step_f  : function). *)
-
-  (*   Hypothesis Getreset_s : Genv.find_symbol tge (prefix_fun main_node reset) = Some rst_ptr. *)
-  (*   Hypothesis Getreset_f : Genv.find_funct_ptr tge rst_ptr = Some (Internal reset_f). *)
-  (*   Hypothesis Getstep_s  : Genv.find_symbol tge (prefix_fun main_node step) = Some stp_ptr. *)
-  (*   Hypothesis Getstep_f  : Genv.find_funct_ptr tge stp_ptr = Some (Internal step_f). *)
-
-  (*   Variables (main_b : block) *)
-  (*             (sb     : block). *)
-
-  (*   Hypothesis Find_s_main : Genv.find_symbol tge tprog.(Ctypes.prog_main) = Some main_b. *)
-  (*   Hypothesis Findmain    : Genv.find_funct_ptr tge main_b = Some (Ctypes.Internal main_f). *)
-
-  (*   Variables (m0 m1: Mem.mem). *)
-  (*   Hypothesis Initmem: Genv.init_mem tprog = Some m0 *)
-  (*                       /\ m0 |= staterep gcenv prog main_node mempty sb Z0. *)
-
-  (*   Hypothesis Hm1: case_out main_step *)
-  (*                            (m1 = m0) *)
-  (*                            (fun _ _ => m1 = m0) *)
-  (*                            (fun _ => *)
-  (*                               exists step_b step_co, *)
-  (*                                 alloc_variables tge empty_env m0 (fn_vars main_f) *)
-  (*                                                 (PTree.set out_step (step_b, t_out_step) empty_env) m1 *)
-  (*                                 /\ gcenv ! (prefix_fun main_node step) = Some step_co *)
-  (*                                 /\ m1 |= staterep gcenv prog main_node mempty sb Z0 *)
-  (*                                          ** blockrep gcenv vempty step_co.(co_members) step_b). *)
-  (*     (*                       end  *) *)
-
-
-  (*     (* Let e1 := case_out main_step *) *)
-  (*     (*                    empty_env *) *)
-  (*     (*                    (fun _ _ => empty_env) *) *)
-  (*     (*                    (fun _ => PTree.set out_step (step_b, t_out_step) empty_env). *) *)
-
-  (*     (*           end. *) *)
-  (*     (* Hypothesis Alloc: alloc_variables tge empty_env m0 main_f.(fn_vars) e1 m1. *) *)
-
-  (*     (* Hypothesis find_step: Genv.find_symbol (Genv.globalenv tprog) (glob_id self) = Some sb. *) *)
-
-  (*     (* Variable P: massert. *) *)
-
-  (*     (* Hypothesis Hm0: m1 |= staterep gcenv prog main_node mempty sb Z0 *) *)
-  (*     (*                    ** match m_step.(m_out) with *) *)
-  (*     (*                       | [] | [_] => sepemp *) *)
-  (*     (*                       | _ => blockrep gcenv vempty step_co.(co_members) step_b *) *)
-  (*     (*                       end *) *)
-  (*     (*                    ** P. *) *)
-
-  (*     Variable me0: menv. *)
-  (*     Hypothesis ResetNode: stmt_call_eval prog mempty main_node reset [] me0 []. *)
-
-  (*     Lemma foo: *)
-  (*       call_spec prog tge c_main main_reset [] [] mempty me0. *)
-  (*     Proof. *)
-  (*       eapply stmt_call_correctness; simpl; eauto. *)
-
-
-  (*       a *)
-  (*       unfold call_spec. *)
-
-  (*     Let le_main := create_undef_temps main_f.(fn_temps). *)
-
-  (*     Lemma entry_main: *)
-  (*       function_entry2 (globalenv tprog) main_f [] m0 e1 le_main m1. *)
-  (*     Proof. *)
-  (*       destruct Caractmain as (Hret & Hcc & Hparams & Hvars & Htemps & Hbody). *)
-  (*       econstructor; eauto. *)
-  (*       - rewrite Hvars. *)
-  (*         unfold var_names. *)
-  (*         rewrite <-NoDup_norepet, <-fst_NoDupMembers. *)
-  (*         destruct_list m_step.(m_out); repeat constructor; auto. *)
-  (*       - rewrite Hparams; constructor. *)
-  (*       - rewrite Hparams, Htemps; simpl. *)
-  (*         intros ? ? Hx; contradiction. *)
-  (*       - unfold le_main; rewrite Hparams, Htemps; simpl; auto. *)
-  (*     Qed. *)
-
-  (*     Lemma match_states_main_after_reset: *)
-  (*       exists m2, *)
-  (*         eval_funcall tge (function_entry2 tge) m1 (Internal reset_f) *)
-  (*                      [var_ptr sb] E0 m2 Vundef *)
-  (*         /\ m2 |= staterep gcenv prog c_main.(c_name) me0 sb 0 *)
-  (*                                                     ** match m_step.(m_out) with *)
-  (*                                                        | [] | [_] => sepemp *)
-  (*                                                        | _ => blockrep gcenv vempty step_co.(co_members) step_b *)
-  (*                                                        end *)
-  (*                                                     ** P. *)
-  (*     Proof. *)
-  (*       pose proof methods_corres as MC. *)
-  (*       pose proof corres_auto_funcall as CAF. *)
-  (*       pose proof (find_class_name _ _ _ _ Find) as Eq; *)
-  (*         pose proof (find_method_name _ _ _ Findreset) as Eq'; *)
-  (*         rewrite <-Eq, <-Eq' in *. *)
-  (*       edestruct MC with (2:=Findreset) *)
-  (*         as (ptr & f & Get_s & Get_f & Hp & ? & ? & ? & ? & ? & ? & ?); eauto. *)
-  (*       rewrite Getreset_s in Get_s; inversion Get_s; subst ptr; *)
-  (*         rewrite Getreset_f in Get_f; inversion Get_f; subst f. *)
-  (*       edestruct CAF with (3:=Findreset) (vs := @nil val) (rvs := @nil val) *)
-  (*         as (m'' & ? & Hm''); eauto. *)
-  (*       - rewrite Reset_out_spec, sep_swap, <-sepemp_left; eauto. *)
-  (*       - rewrite Reset_in_spec; auto. *)
-  (*       - rewrite Hp, Reset_in_spec, Reset_out_spec; auto. *)
-  (*       - rewrite Reset_out_spec; auto. *)
-  (*       - edestruct wt_program_find_class as [WT_main]; eauto. *)
-  (*         eapply wt_stmt_sub with (prog':=prog_main); eauto. *)
-  (*         + eapply wt_class_find_method with (2:=Findreset); auto. *)
-  (*         + eapply find_class_sub; eauto. *)
-  (*       - rewrite Reset_out_spec in *. *)
-  (*         exists m''; split; auto. *)
-  (*         rewrite sep_swap, <-sepemp_left in Hm''; auto. *)
-
-  (*         Grab Existential Variables. *)
-  (*         eauto. *)
-  (*         eauto. *)
-  (*     Qed. *)
-
-  (*     Lemma match_states_main_after_step: *)
-  (*       forall m' P me me' vs rvs, *)
-  (*         stmt_call_eval prog me c_main.(c_name) m_step.(m_name) (map Some vs) me' (map Some rvs) -> *)
-  (*         m' |= staterep gcenv prog c_main.(c_name) me sb 0 *)
-  (*                                                   ** match m_step.(m_out) with *)
-  (*                                                      | [] | [_] => sepemp *)
-  (*                                                      | _ => blockrep gcenv vempty step_co.(co_members) step_b *)
-  (*                                                      end *)
-  (*                                                   ** P -> *)
-  (*         wt_mem me prog_main c_main -> *)
-  (*         wt_vals vs m_step.(m_in) -> *)
-  (*         exists m'', *)
-  (*           eval_funcall tge (function_entry2 tge) m' (Internal step_f) *)
-  (*                        (var_ptr sb *)
-  (*                              :: match m_step.(m_out) with *)
-  (*                                | [] | [_] => vs *)
-  (*                                | _ => var_ptr step_b :: vs *)
-  (*                                end) E0 m'' *)
-  (*                        match rvs with *)
-  (*                        | [v] => v *)
-  (*                        | _ => Vundef *)
-  (*                        end *)
-
-  (*           /\ m'' |= staterep gcenv prog c_main.(c_name) me' sb 0 *)
-  (*                                                        ** match m_step.(m_out) with *)
-  (*                                                           | [] | [_] => sepemp *)
-  (*                                                           | _ => blockrep gcenv (Env.adds (map fst m_step.(m_out)) rvs vempty) step_co.(co_members) step_b *)
-  (*                                                           end *)
-  (*                                                        ** P. *)
-  (*     Proof. *)
-  (*       pose proof methods_corres as MC. *)
-  (*       pose proof corres_auto_funcall as CAF. *)
-  (*       intros. *)
-  (*       pose proof (find_class_name _ _ _ _ Find) as Eq; *)
-  (*         pose proof (find_method_name _ _ _ Findstep) as Eq'; *)
-  (*         rewrite <-Eq, <-Eq' in *. *)
-  (*       edestruct MC with (2:=Findstep) *)
-  (*         as (ptr & f & Get_s & Get_f & Hp & ? & ? & ? & ? & ? & ? & ?); eauto. *)
-  (*       rewrite Getstep_s in Get_s; inversion Get_s; subst ptr; *)
-  (*         rewrite Getstep_f in Get_f; inversion Get_f; subst f. *)
-  (*       edestruct CAF with (3:=Findstep) as (m'' & ? & Hm''); eauto. *)
-  (*       - destruct_list m_step.(m_out); rewrite Hp; simpl; rewrite map_length; *)
-  (*           symmetry; erewrite Forall2_length; eauto. *)
-  (*       - edestruct wt_program_find_class as [WT_main]; eauto. *)
-  (*         eapply wt_stmt_sub with (prog':=prog_main); eauto. *)
-  (*         + eapply wt_class_find_method with (2:=Findstep); auto. *)
-  (*         + eapply find_class_sub; eauto. *)
-  (*     Qed. *)
-
-
-  (*     (*****************************************************************) *)
-  (*     (** Trace semantics of reads and writes to volatiles             *) *)
-  (*     (*****************************************************************) *)
-
-  (*     Lemma exec_read: *)
-  (*       forall cs le m, *)
-  (*         wt_vals cs m_step.(m_in) -> *)
-  (*         exists le', (* XXX: not any le': the one that contains [cs] *) *)
-  (*           exec_stmt (globalenv tprog) (function_entry2 (globalenv tprog)) e1 le m *)
-  (*                     (load_in m_step.(m_in)) *)
-  (*                     (load_events cs m_step.(m_in)) *)
-  (*                     le' m Out_normal *)
-  (*           /\ Forall2 (fun v xt => le' ! (fst xt) = Some v) cs m_step.(m_in) *)
-  (*           /\ (forall x, ~ InMembers x m_step.(m_in) -> le' ! x = le ! x). *)
-  (*     Proof. *)
-  (*       clear Caractmain Step_in_spec. *)
-  (*       pose proof (m_nodupin m_step) as Hnodup. *)
-  (*       pose proof (m_good_in m_step) as Good. *)
-
-  (*       induction m_step.(m_in) as [|(x, t)]; simpl; *)
-  (*         intros * Hwt; *)
-  (*         inversion_clear Hwt as [| v ? vs ? Hwt_v Hwts ]; *)
-  (*         inversion_clear Hnodup. *)
-  (*       - (* Case: m_step.(m_in) ~ [] *) *)
-  (*         rewrite load_events_nil. *)
-  (*         repeat econstructor; auto. *)
-  (*       - (* Case: m_step.(m_in) ~ xt :: xts *) *)
-  (*         inversion_clear Step_in as [|? ? Findx]. *)
-  (*         destruct Findx as (bx & Findx & Volx). *)
-  (*         rewrite load_events_cons. *)
-
-  (*         assert (exists le', *)
-  (*                    exec_stmt (globalenv tprog) (function_entry2 (globalenv tprog)) e1 le m *)
-  (*                              (Sbuiltin (Some x) (AST.EF_vload (type_chunk t)) *)
-  (*                                        (Ctypes.Tcons (Tpointer (cltype t) noattr) Ctypes.Tnil) *)
-  (*                                        [Eaddrof (Evar (glob_id x) (cltype t)) (Tpointer (cltype t) noattr)]) *)
-  (*                              [load_event_of_val v (x, t)] le' m Out_normal *)
-  (*                    /\ le' ! x = Some v *)
-  (*                    /\ forall y, y <> x -> le' ! y = le ! y) *)
-  (*           as (le' & Hload & Hgss_le' & Hgso_le'). *)
-  (*         { *)
-  (*           exists (set_opttemp (Some x) v le). *)
-  (*           repeat split; *)
-  (*             [ *)
-  (*             | now apply  PTree.gss *)
-  (*             | now intros; eapply PTree.gso ]. *)
-  (*           econstructor. *)
-  (*           - econstructor; eauto using eval_exprlist. *)
-  (*             + apply eval_Eaddrof, eval_Evar_global; eauto. *)
-  (*               rewrite <-not_Some_is_None. *)
-  (*               intros (b, t') Hget. *)
-  (*               subst e1. *)
-  (*               assert (glob_id x <> self) by (eapply self_not_glob; eauto). *)
-  (*               destruct_list m_step.(m_out). *)
-  (*               * rewrite PTree.gempty in Hget; auto; try discriminate. *)
-  (*               * rewrite PTree.gempty in Hget; auto; try discriminate. *)
-  (*               *{ rewrite PTree.gso, PTree.gempty in Hget; auto; try discriminate. *)
-  (*                  intro E; apply (glob_id_not_prefixed x). *)
-  (*                  - apply (Good (x, t)), in_eq. *)
-  (*                  - rewrite E; constructor. *)
-  (*                } *)
-  (*             + unfold Cop.sem_cast; simpl; eauto. *)
-  (*           - constructor. *)
-  (*             unfold load_event_of_val; simpl. *)
-  (*             rewrite wt_val_load_result with (ty:=t); auto. *)
-  (*             apply volatile_load_vol; auto. *)
-  (*             apply eventval_of_val_match; auto. *)
-  (*         } *)
-
-  (*         assert (forall x0 : ident * type, In x0 l -> ValidId x0) *)
-  (*           by (intros; apply Good, in_cons; auto). *)
-  (*         edestruct IHl with (le := le') as (le'' & ? & Hgss & Hgso); eauto. *)
-
-  (*         exists le''. *)
-  (*         repeat split. *)
-  (*         + eapply exec_Sseq_1; eauto. *)
-  (*         + econstructor; eauto. *)
-  (*           rewrite Hgso; auto. *)
-  (*         + intros * Hnot_in. *)
-  (*           apply Decidable.not_or in Hnot_in as [? ?]. *)
-  (*           rewrite Hgso; auto. *)
-  (*     Qed. *)
-
-  (*     Lemma exec_write: *)
-  (*       forall vs ve le m, *)
-  (*         wt_vals vs m_step.(m_out) -> *)
-  (*         m |= match m_step.(m_out), vs with *)
-  (*              | [], [] => sepemp *)
-  (*              | [(y, _)], [v] => pure (le ! y = Some v) *)
-  (*              | _, _ => blockrep gcenv (Env.adds (map fst m_step.(m_out)) vs ve) (co_members step_co) step_b *)
-  (*              end *)
-  (*           ** P -> *)
-  (*         exec_stmt (globalenv tprog) (function_entry2 (globalenv tprog)) e1 le m *)
-  (*                   (write_out main_node m_step.(m_out)) *)
-  (*                   (store_events vs m_step.(m_out)) *)
-  (*                   le m Out_normal. *)
-  (*     Proof. *)
-  (*       pose proof global_out_struct as GOS. *)
-  (*       intros * WT_vals Hrep. *)
-  (*       assert (length vs = length m_step.(m_out)) as Length by (eapply Forall2_length; eauto). *)
-  (*       (* XXX: factorize proof (& code) with [exec_read] *) *)
-  (*       destruct_list m_step.(m_out) as (y, t) (y', t') outs : Out; *)
-  (*         destruct_list vs as v v' vs' : Vs; contr. *)
-
-  (*       - unfold write_out. *)
-  (*         inversion_clear Step_out as [|? ? Findy]. *)
-  (*         destruct Findy as (b_y & Findy & Voly). *)
-  (*         inversion_clear WT_vals. *)
-  (*         eapply exec_Sbuiltin with (vres:=Vundef). *)
-  (*         + repeat *)
-  (*             match goal with *)
-  (*             | |- eval_exprlist _ _ _ _ _ _ _ => econstructor *)
-  (*             end. *)
-  (*           * econstructor. *)
-  (*             apply eval_Evar_global; eauto. *)
-  (*             rewrite <-not_Some_is_None. *)
-  (*             intros (b, t'') Hget. *)
-  (*             subst e1. *)
-  (*             rewrite PTree.gempty in Hget; contr. *)
-  (*           * reflexivity. *)
-  (*           * econstructor. *)
-  (*             apply sep_pure in Hrep; destruct Hrep as (Hpure & Hrep). *)
-  (*             change val with Values.val in Hpure. *)
-  (*             rewrite Hpure; eauto. *)
-  (*           * eapply sem_cast_same; eauto. *)
-  (*         + constructor. *)
-  (*           apply volatile_store_vol; auto; simpl. *)
-  (*           rewrite <-wt_val_load_result; auto. *)
-  (*           apply eventval_of_val_match; auto. *)
-
-  (*       - assert (1 < length m_step.(m_out))%nat by (rewrite Out; simpl; omega). *)
-  (*         clear Caractmain Step_out_spec Hm0. *)
-
-  (*         pose proof (m_nodupout m_step) as Hnodup. *)
-
-  (*         pose proof (find_class_name _ _ _ _ Find) as Eq; *)
-  (*           pose proof (find_method_name _ _ _ Findstep) as Eq'; *)
-  (*           rewrite <-Eq, <-Eq' in *. *)
-
-  (*         assert (e1 ! (prefix out step) *)
-  (*                 = Some (step_b, type_of_inst (prefix_fun main_node step))) as Findstr *)
-  (*             by (subst e1; rewrite PTree.gss; auto). *)
-  (*         rewrite <-Eq, <-Eq' in Findstr. *)
-
-  (*         edestruct GOS with (2:=Findstep) *)
-  (*           as (step_co' & Hrco & ? & Hmr & ? & ? & ?); eauto. *)
-  (*         rewrite Getstep_co in Hrco; inversion Hrco; subst step_co'. *)
-
-  (*         (* This induction is tricky: [co_members step_co ~ m_out m_step] *)
-  (*          is fixed across the induction while we are going down inside *)
-  (*          [m_out m_step]. The following assertion allows us to get back *)
-  (*          into [co_members] whenever necessary. *) *)
-
-  (*         assert (Hfield_offs: forall x ty, *)
-  (*                    In (x, ty) (map translate_param (m_out m_step)) -> *)
-  (*                    In (x, ty) (co_members step_co)) *)
-  (*           by now rewrite Hmr. *)
-
-  (*         unfold write_out. *)
-
-  (*         rewrite <-Vs, <-Out in *. *)
-  (*         clear Vs. *)
-  (*         pose proof (m_good_out m_step) as Good. *)
-  (*         revert ve vs Hrep Hnodup Hfield_offs Findstr Step_out Eq Eq' Length WT_vals Good. *)
-  (*         generalize m_step.(m_out) as xts. *)
-  (*         clear - Getstep_co. *)
-
-  (*         induction xts as [|(x, t) xts]; destruct vs; contr; *)
-  (*           intros; eauto using exec_stmt. *)
-
-  (*         inversion_clear Hnodup as [|? ? ? Notin]. *)
-  (*         inversion_clear Step_out as [|? ? Findx]. *)
-  (*         destruct Findx as (bx & Findx & Volx). *)
-  (*         inversion_clear WT_vals. *)
-
-  (*         rewrite store_events_cons. *)
-  (*         eapply exec_Sseq_1 with (le1 := le); eauto. *)
-  (*         + eapply exec_Sbuiltin with (vres:=Vundef). *)
-  (*           *{ repeat *)
-  (*                match goal with *)
-  (*                | |- eval_exprlist _ _ _ _ _ _ _ => econstructor *)
-  (*                end. *)
-  (*              - econstructor. *)
-  (*                apply eval_Evar_global; eauto. *)
-  (*                rewrite <-not_Some_is_None. *)
-  (*                intros (b, t'') Hget. *)
-  (*                subst e1. *)
-  (*                rewrite PTree.gso, PTree.gempty in Hget. *)
-  (*                + discriminate. *)
-  (*                + intro E; apply (glob_id_not_prefixed x). *)
-  (*                  * apply (Good (x, t)), in_eq. *)
-  (*                  * rewrite E; constructor. *)
-  (*              - reflexivity. *)
-  (*              - assert (In (x, cltype t) (co_members step_co)) *)
-  (*                  by now eapply Hfield_offs; econstructor; eauto. *)
-
-  (*                edestruct blockrep_field_offset as (? & ? & ? & ?); eauto. *)
-
-  (*                eapply eval_Elvalue; eauto. *)
-  (*                + eapply eval_Efield_struct; eauto. *)
-  (*                  *{ eapply eval_Elvalue; eauto. *)
-  (*                     - constructor; *)
-  (*                         rewrite <- Eq'; eauto. *)
-  (*                     - now apply deref_loc_copy. *)
-  (*                   } *)
-  (*                  * unfold type_of_inst; simpl; rewrite Eq'; eauto. *)
-  (*                + simpl; eapply blockrep_deref_mem; eauto. *)
-  (*                  * simpl; apply Env.find_gsss. *)
-  (*                    now rewrite <-fst_InMembers. *)
-  (*                  * rewrite Ptrofs.unsigned_zero; simpl. *)
-  (*                    rewrite Ptrofs.unsigned_repr; auto. *)
-  (*              - eapply sem_cast_same; eauto. *)
-  (*            } *)
-  (*           * constructor. *)
-  (*             apply volatile_store_vol; auto. *)
-  (*             rewrite <-wt_val_load_result; auto. *)
-  (*             apply eventval_of_val_match; auto. *)
-
-  (*         + eapply IHxts with (ve:=Env.add x v ve); eauto. *)
-  (*           * intros. *)
-  (*             eapply Hfield_offs. constructor 2; auto. *)
-  (*           * intros; apply Good, in_cons; auto. *)
-  (*     Qed. *)
 
   (*****************************************************************)
   (** Clight version of dostep                                    **)
@@ -2407,24 +1639,25 @@ Section PRESERVATION.
 
 
     CoInductive dostep (e: Clight.env) : nat -> mem -> Prop :=
-      Step :
+      DoStep :
         forall n m m',
           case_out main_step
-                   (eval_funcall tge (function_entry2 tge) m (Internal step_f)
+                   (eval_funcall_fe function_entry2 tge m (Internal step_f)
                                  (var_ptr sb :: ins n) E0 m' Vundef)
                    (fun _ _ =>
                       exists v,
                         outs n = [v]
-                        /\ eval_funcall tge (function_entry2 tge) m (Internal step_f)
+                        /\ eval_funcall_fe function_entry2 tge m (Internal step_f)
                                        (var_ptr sb :: ins n) E0 m' v)
                    (fun ys =>
                       exists ve step_b step_co,
-                        eval_funcall tge (function_entry2 tge) m (Internal step_f)
+                        eval_funcall_fe function_entry2 tge m (Internal step_f)
                                      (var_ptr sb :: var_ptr step_b :: ins n) E0 m' Vundef
                           /\ gcenv ! (prefix_fun main_node step) = Some step_co
                         /\ e ! out_step = Some (step_b, t_out_step)
                         /\ Forall2 (fun xt v => Env.find (fst xt) ve = Some v) ys (outs n)
                         /\ m' |= blockrep gcenv ve (co_members step_co) step_b) ->
+          out_step_env e ->
           dostep e (S n) m' ->
           dostep e n m.
 
@@ -2433,21 +1666,23 @@ Section PRESERVATION.
       Variable R: nat -> mem -> Prop.
       Variable e: Clight.env.
 
+      Hypothesis He : out_step_env e.
+
       Definition dostepCase :=
         forall n m,
           R n m ->
           exists m',
             case_out main_step
-                     (eval_funcall tge (function_entry2 tge) m (Internal step_f)
+                     (eval_funcall_fe function_entry2 tge m (Internal step_f)
                                    (var_ptr sb :: ins n) E0 m' Vundef)
                      (fun _ _ =>
                       exists v,
                         outs n = [v]
-                        /\ eval_funcall tge (function_entry2 tge) m (Internal step_f)
+                        /\ eval_funcall_fe function_entry2 tge m (Internal step_f)
                                        (var_ptr sb :: ins n) E0 m' v)
                      (fun ys =>
                         exists ve step_b step_co,
-                          eval_funcall tge (function_entry2 tge) m (Internal step_f)
+                          eval_funcall_fe function_entry2 tge m (Internal step_f)
                                        (var_ptr sb :: var_ptr step_b :: ins n) E0 m' Vundef
                           /\ gcenv ! (prefix_fun main_node step) = Some step_co
                           /\ e ! out_step = Some (step_b, t_out_step)
@@ -2470,168 +1705,59 @@ Section PRESERVATION.
 
     End Dostep_coind.
 
-    (*****************************************************************)
-    (** Correctness of dostep relatively to loop_call               **)
-    (*****************************************************************)
-
-    Lemma dostep_imp:
-      forall reset_f m_init me0 e,
-        method_spec c_main main_reset prog reset_f ->
-        case_out main_step
-                 (m_init |= staterep gcenv prog main_node mempty sb Z0)
-                 (fun _ _ =>
-                    m_init |= staterep gcenv prog main_node mempty sb Z0)
-                 (fun _ =>
-                    exists step_b step_co,
-                      gcenv ! (prefix_fun main_node step) = Some step_co
-                      /\ e ! out_step = Some (step_b, t_out_step)
-                      /\ m_init |= staterep gcenv prog main_node mempty sb Z0
-                                  ** blockrep gcenv vempty step_co.(co_members) step_b) ->
-        stmt_call_eval prog mempty main_node reset [] me0 [] ->
-        wt_mem me0 prog_main c_main ->
-        loop_call prog main_node step (fun n => map Some (ins n)) (fun n => map Some (outs n)) 0 me0 ->
-        exists m0,
-          eval_funcall tge (function_entry2 tge) m_init (Internal reset_f)
-                       [var_ptr sb] E0 m0 Vundef
-          /\ dostep e 0 m0.
-    Proof.
-      intros * SpecReset Hm_init EvalReset WTm Loop.
-
-      (* reset correctness preparation *)
-      assert (m_out main_reset = []) as Hout_reset.
-      { inversion_clear EvalReset as [??????????? Findcl Findmth ?? Houts].
-        rewrite find_main_class in Findcl; inv Findcl;
-          rewrite find_main_reset in Findmth; inv Findmth.
-        rewrite Forall2_map_1 in Houts; unfold main_reset; inv Houts; auto.
-      }
-      apply reset_correct in EvalReset.
-      unfold call_spec, case_out in EvalReset.
-      rewrite Hout_reset in EvalReset.
-      erewrite find_class_name in EvalReset; eauto.
-      rewrite <- Ptrofs.unsigned_zero in Hm_init.
-
-      (* prepare the coinduction relation in advance *)
-      set (R := fun n m => case_out main_step
-                                 (exists me,
-                                     loop_call prog main_node step
-                                               (fun n => map Some (ins n)) (fun n => map Some (outs n)) n me
-                                     /\ wt_mem me prog_main c_main
-                                     /\ m |= staterep gcenv prog main_node me sb 0)
-                                 (fun _ _ =>
-                                    exists me,
-                                      loop_call prog main_node step
-                                                (fun n => map Some (ins n)) (fun n => map Some (outs n)) n me
-                                      /\ wt_mem me prog_main c_main
-                                      /\ m |= staterep gcenv prog main_node me sb 0 )
-                                 (fun _ =>
-                                    exists me step_b step_co,
-                                      loop_call prog main_node step
-                                                (fun n => map Some (ins n)) (fun n => map Some (outs n)) n me
-                                      /\ wt_mem me prog_main c_main
-                                      /\ gcenv ! (prefix_fun main_node step) = Some step_co
-                                      /\ e ! out_step = Some (step_b, t_out_step)
-                                      /\ m |= staterep gcenv prog main_node me sb 0
-                                          ** blockrep gcenv vempty (co_members step_co) step_b)).
-
-      assert (dostepCase R e).
-      { unfold R; unfold dostepCase, case_out.
-        intros n m_n Spec.
-        destruct_list (m_out main_step) as (?,?) (?,?) ? : Hout;
-          [destruct Spec as (? & Dostep & Hwt & Hm_n)
-          |destruct Spec as (? & Dostep & Hwt & Hm_n)
-          |destruct Spec as (? & step_b' & step_co' & Dostep & Hwt & ? & ? & Hm_n)];
-          destruct Dostep as [? me_n me_Sn EvalStep dostep];
-          assert (wt_mem me_Sn prog_main c_main)
-            by (eapply pres_sem_stmt_call with (f := step); eauto;
-                rewrite Forall2_map_1; simpl; apply Hwt_ins);
-
-          (* step correctness *)
-          eapply step_correct in EvalStep; auto;
-          unfold call_spec, case_out in EvalStep;
-          rewrite Hout in EvalStep; erewrite find_class_name in EvalStep; eauto;
-            rewrite sepemp_right, <- Ptrofs.unsigned_zero in Hm_n; try rewrite sep_assoc in Hm_n;
-              [eapply EvalStep in Hm_n as (m_Sn & step_f' & ? & ? & Hm_Sn)
-              |eapply EvalStep in Hm_n as (m_Sn & step_f' & ? & ? & ? & ? & Hm_Sn)
-              |eapply EvalStep in Hm_n as (ve_f & m_Sn & step_f' & ? & ? & ? & Hm_Sn)]; auto;
-                try erewrite find_method_name; eauto;
-                  assert (step_f = step_f') by (eapply method_spec_eq; eauto); subst step_f'.
-
-        - exists m_Sn; split; eauto.
-          exists me_Sn; intuition.
-          now rewrite <-sepemp_right, Ptrofs.unsigned_zero in Hm_Sn.
-        - exists m_Sn; split; eauto.
-          exists me_Sn; intuition.
-          now rewrite <-sepemp_right, Ptrofs.unsigned_zero in Hm_Sn.
-        - exists m_Sn; split; eauto.
-          + exists ve_f, step_b', step_co'; intuition.
-            now apply sep_proj2, sep_proj1 in Hm_Sn.
-          + exists me_Sn, step_b', step_co'; intuition.
-            rewrite <-sepemp_right, Ptrofs.unsigned_zero in Hm_Sn.
-            eapply sep_imp; eauto.
-            apply blockrep_any_empty.
-      }
-
-      unfold case_out in Hm_init.
-      destruct_list (m_out main_step) as (?,?) (?,?) ? : Hout;
-
-        (* reset correctness *)
-        [rewrite sepemp_right in Hm_init
-        |rewrite sepemp_right in Hm_init
-        |destruct Hm_init as (step_b & step_co & ? & ? & Hm_init)];
-        eapply EvalReset in Hm_init as (m0 & reset_f' & ? & ? & Hm0); auto;
-          assert (reset_f = reset_f') by (eapply method_spec_eq; eauto); subst reset_f';
-            exists m0; split; auto;
-
-              (* loop correctness using the R relation defined before *)
-              apply dostep_coind with (R := R); auto;
-                unfold R, case_out; rewrite Hout.
-      - exists me0; intuition.
-        now rewrite <-sepemp_right, Ptrofs.unsigned_zero in Hm0.
-      - exists me0; intuition.
-        now rewrite <-sepemp_right, Ptrofs.unsigned_zero in Hm0.
-      - exists me0, step_b, step_co; intuition.
-    Qed.
-
 
     (*****************************************************************)
-    (** Correctness of the main loop relatively to dostep           **)
+    (** dostep implies a step of the body loop                      **)
     (*****************************************************************)
 
-    Remark prefix_out_env_no_prefix_fun:
+    Hypothesis Hwt_outs : forall n, wt_vals (outs n) main_step.(m_out).
+
+    Remark out_step_env_no_prefix_fun:
       forall e x f,
-        prefix_out_env e ->
+        out_step_env e ->
         e ! (prefix_fun x f) = None.
     Proof.
       intros * He.
       rewrite <-not_Some_is_None.
       intros (b, t') Hget.
-      apply He in Hget as (?&?& E).
-      eapply prefix_fun_not_out; eauto.
+      apply He in Hget; unfold out_step in Hget.
+      unfold prefix_fun in Hget.
+      apply prefix_injective in Hget as (?&?); auto using fun_id_valid, out_valid.
     Qed.
-    Hint Resolve prefix_out_env_no_prefix_fun.
+    Hint Resolve out_step_env_no_prefix_fun.
 
     Let step_name := Evar (prefix_fun main_node step).
     Let self_addr := Eaddrof (Evar (glob_id self) (type_of_inst main_node))
-                             (type_of_inst_p main_node).
+                               (type_of_inst_p main_node).
+
+    (** evaluate the self parameter *)
+    Lemma eval_expr_self:
+      forall e le m,
+        out_step_env e ->
+        eval_expr tge e le m self_addr (var_ptr sb).
+    Proof.
+      econstructor.
+      apply eval_Evar_global; eauto.
+      apply out_step_env_no_glob_id; auto; apply self_valid.
+    Qed.
+    Hint Resolve eval_expr_self.
 
     Lemma exec_body:
-      forall n m_n le_n e,
-        wt_vals (outs n) (m_out main_step) ->
-        prefix_out_env e ->
+      forall e n m_n le_n,
         dostep e n m_n ->
         exists le_Sn m_Sn,
-          exec_stmt (globalenv tprog) (function_entry2 (globalenv tprog)) e le_n m_n
-                    (main_loop_body false main_node main_step)
-                    (load_events (ins n) (m_in main_step)
-                                 ++ E0
-                                 ++ store_events (outs n) (m_out main_step))
-                    le_Sn m_Sn Out_normal
+          exec_stmt_fe function_entry2 tge e le_n m_n
+                       (main_loop_body false main_node main_step)
+                       (load_events (ins n) (m_in main_step)
+                         ++ E0
+                         ++ store_events (outs n) (m_out main_step))
+                       le_Sn m_Sn Out_normal
           /\ dostep e (S n) m_Sn.
     Proof.
-      intros * WTouts He Hdostep.
+      intros * Dostep.
 
       (* the loop predicate gives the expected memory after a call *)
-      inversion_clear Hdostep as [?? m_Sn EvalStep].
+      inversion_clear Dostep as [?? m_Sn EvalStep].
 
       (*  load in *)
       edestruct exec_read with (le := le_n) (m := m_n) as (le1 & ?&?&?); eauto.
@@ -2646,13 +1772,6 @@ Section PRESERVATION.
       { intros; eapply eval_Elvalue.
         - apply eval_Evar_global; eauto.
         - apply deref_loc_reference; auto.
-      }
-
-      (* evaluate the self parameter *)
-      assert (eval_expr tge e le1 m_n self_addr (var_ptr sb)).
-      { econstructor.
-        apply eval_Evar_global; eauto.
-        apply prefix_out_env_no_glob_id; auto; apply self_valid.
       }
 
       (* evaluate the arguments of the step call *)
@@ -2680,14 +1799,14 @@ Section PRESERVATION.
 
       (* step call *)
       assert (exists le2,
-                 exec_stmt tge (function_entry2 tge) e le1 m_n
+                 exec_stmt_fe function_entry2 tge e le1 m_n
                            (step_call main_node (map make_in_arg (m_in main_step)) (m_out main_step))
                            E0 le2 m_Sn Out_normal
                  /\ match main_step.(m_out), outs n with
                    | [(x, _)], [v] => le2 ! x = Some v
                    | _, _ => True
                    end)
-            as (le2 & Hcall & ?).
+        as (le2 & Hcall & ?).
       { unfold step_call.
         destruct_list main_step.(m_out) as (?, ?) ? ? : Out;
           unfold case_out in EvalStep; rewrite Out in EvalStep.
@@ -2709,7 +1828,7 @@ Section PRESERVATION.
           + simpl; apply PTree.gss.
         - destruct EvalStep as (?&?&?&?&?&?&?).
           eexists; split; auto.
-          eapply exec_Scall; simpl; eauto; simpl; eauto 6 using eval_exprlist.
+          eapply exec_Scall; simpl; eauto; simpl; eauto 7 using eval_exprlist.
           unfold type_of_function.
           destruct StepSpec as (P_f & R_f & CC_f &?).
           rewrite P_f, R_f, CC_f; unfold case_out; rewrite Out; simpl.
@@ -2731,242 +1850,343 @@ Section PRESERVATION.
         exists ve, step_b, step_co; intuition; eauto.
     Qed.
 
-    Definition transl_trace (n: nat): traceinf' :=
-      trace_step m_step ins outs Step_in_spec Step_out_spec Hwt_ins Hwt_outs n.
+    Section MainCorrectness.
+
+      Variables (me0     : menv)
+                (reset_f : function)
+                (e       : Clight.env)
+                (m_main  : mem).
+
+      Hypothesis (ResetCall : stmt_call_eval prog mempty main_node reset [] me0 [])
+                 (WTme0     : wt_mem me0 prog_main c_main)
+                 (StepLoop  : loop_call prog main_node step (fun n => map Some (ins n)) (fun n => map Some (outs n)) 0 me0)
+                 (ResetSpec : method_spec c_main main_reset prog reset_f)
+                 (He        : out_step_env e)
+                 (Hm_main   : if lt_dec 1 (length (m_out main_step))
+                              then
+                                exists step_b step_co,
+                                  gcenv ! (prefix_fun main_node step) = Some step_co
+                                  /\ e ! out_step = Some (step_b, t_out_step)
+                                  /\ m_main |= staterep gcenv prog main_node mempty sb Z0
+                                           ** blockrep gcenv vempty step_co.(co_members) step_b
+                              else m_main |= staterep gcenv prog main_node mempty sb Z0).
+
+      Lemma reset_no_output:
+        m_out main_reset = [].
+      Proof.
+        inversion_clear ResetCall as [??????????? Findcl Findmth ?? Houts].
+        rewrite find_main_class in Findcl; inv Findcl;
+          rewrite find_main_reset in Findmth; inv Findmth.
+        rewrite Forall2_map_1 in Houts; unfold main_reset; inv Houts; auto.
+      Qed.
+
+      Lemma reset_no_input:
+        m_in main_reset = [].
+      Proof.
+        inversion_clear ResetCall as [??????????? Findcl Findmth].
+        rewrite find_main_class in Findcl; inv Findcl;
+          rewrite find_main_reset in Findmth; inv Findmth.
+        destruct main_reset.(m_in); simpl in *; auto; omega.
+      Qed.
+
+      (*****************************************************************)
+      (** Correctness of dostep relatively to loop_call               **)
+      (*****************************************************************)
+
+      Lemma dostep_imp:
+        exists m0,
+          eval_funcall_fe function_entry2 tge m_main (Internal reset_f)
+                          [var_ptr sb] E0 m0 Vundef
+          /\ dostep e 0 m0.
+      Proof.
+        (* reset correctness preparation *)
+        pose proof ResetCall as ResetCall'.
+        apply reset_correct in ResetCall'.
+        unfold call_spec, case_out in ResetCall'.
+        rewrite reset_no_output in ResetCall'.
+        erewrite find_class_name in ResetCall'; eauto.
+        rewrite <- Ptrofs.unsigned_zero in Hm_main.
+
+        (* prepare the coinduction relation in advance *)
+        set (R := fun n m => case_out main_step
+                                   (exists me,
+                                       loop_call prog main_node step
+                                                 (fun n => map Some (ins n)) (fun n => map Some (outs n)) n me
+                                       /\ wt_mem me prog_main c_main
+                                       /\ m |= staterep gcenv prog main_node me sb 0)
+                                   (fun _ _ =>
+                                      exists me,
+                                        loop_call prog main_node step
+                                                  (fun n => map Some (ins n)) (fun n => map Some (outs n)) n me
+                                        /\ wt_mem me prog_main c_main
+                                        /\ m |= staterep gcenv prog main_node me sb 0 )
+                                   (fun _ =>
+                                      exists me step_b step_co,
+                                        loop_call prog main_node step
+                                                  (fun n => map Some (ins n)) (fun n => map Some (outs n)) n me
+                                        /\ wt_mem me prog_main c_main
+                                        /\ gcenv ! (prefix_fun main_node step) = Some step_co
+                                        /\ e ! out_step = Some (step_b, t_out_step)
+                                        /\ m |= staterep gcenv prog main_node me sb 0
+                                            ** blockrep gcenv vempty (co_members step_co) step_b)).
+
+        assert (dostepCase R e).
+        { unfold R; unfold dostepCase, case_out.
+          intros n m_n Spec.
+          destruct_list (m_out main_step) as (?,?) (?,?) ? : Hout;
+            [destruct Spec as (? & Dostep & Hwt & Hm_n)
+            |destruct Spec as (? & Dostep & Hwt & Hm_n)
+            |destruct Spec as (? & step_b' & step_co' & Dostep & Hwt & ? & ? & Hm_n)];
+            destruct Dostep as [? me_n me_Sn EvalStep dostep];
+            assert (wt_mem me_Sn prog_main c_main)
+              by (eapply pres_sem_stmt_call with (f := step); eauto;
+                  rewrite Forall2_map_1; simpl; apply Hwt_ins);
+
+            (* step correctness *)
+            eapply step_correct in EvalStep; auto;
+              unfold call_spec, case_out in EvalStep;
+              rewrite Hout in EvalStep; erewrite find_class_name in EvalStep; eauto;
+                rewrite sepemp_right, <- Ptrofs.unsigned_zero in Hm_n; try rewrite sep_assoc in Hm_n;
+                  [eapply EvalStep in Hm_n as (m_Sn & step_f' & ? & ? & Hm_Sn)
+                  |eapply EvalStep in Hm_n as (m_Sn & step_f' & ? & ? & ? & ? & Hm_Sn)
+                  |eapply EvalStep in Hm_n as (ve_f & m_Sn & step_f' & ? & ? & ? & Hm_Sn)]; auto;
+                    try erewrite find_method_name; eauto;
+                      assert (step_f = step_f') by (eapply method_spec_eq; eauto); subst step_f'.
+
+          - exists m_Sn; split; eauto.
+            exists me_Sn; intuition.
+            now rewrite <-sepemp_right, Ptrofs.unsigned_zero in Hm_Sn.
+          - exists m_Sn; split; eauto.
+            exists me_Sn; intuition.
+            now rewrite <-sepemp_right, Ptrofs.unsigned_zero in Hm_Sn.
+          - exists m_Sn; split; eauto.
+            + exists ve_f, step_b', step_co'; intuition.
+              now apply sep_proj2, sep_proj1 in Hm_Sn.
+            + exists me_Sn, step_b', step_co'; intuition.
+              rewrite <-sepemp_right, Ptrofs.unsigned_zero in Hm_Sn.
+              eapply sep_imp; eauto.
+              apply blockrep_any_empty.
+        }
+
+        cases;
+          (* reset correctness *)
+          [destruct Hm_main as (step_b & step_co & ? & ? & Hm_main');
+           clear Hm_main; rename Hm_main' into Hm_main
+          |rewrite sepemp_right in Hm_main];
+          eapply ResetCall' in Hm_main as (m0 & reset_f' & ? & ? & Hm0); auto;
+            assert (reset_f = reset_f') by (eapply method_spec_eq; eauto); subst reset_f';
+              exists m0; split; auto;
+
+                (* loop correctness using the R relation defined before *)
+                apply dostep_coind with (R := R); auto;
+                  unfold R, case_out; destruct_list (m_out main_step) as (?,?) (?,?) ?;
+                                                                               simpl in *; try omega.
+        - exists me0, step_b, step_co; intuition.
+        - exists me0; intuition.
+          now rewrite <-sepemp_right, Ptrofs.unsigned_zero in Hm0.
+        - exists me0; intuition.
+          now rewrite <-sepemp_right, Ptrofs.unsigned_zero in Hm0.
+      Qed.
+
+      Let reset_name := Evar (prefix_fun main_node reset).
+
+      Corollary exec_reset:
+        exists m0,
+          exec_stmt_fe function_entry2 tge e
+                       le_main m_main (reset_call main_node) E0
+                       le_main m0 Out_normal
+          /\ dostep e 0 m0.
+      Proof.
+        destruct dostep_imp as (m0 & ?&?).
+        exists m0; split; auto.
+
+        (* get the function *)
+        edestruct methods_corres with (4 := find_main_reset) as (ptr_reset & f & Get_s & Get_f & ?); eauto.
+        assert (f = reset_f) by (eapply method_spec_eq; eauto); subst f.
+
+        (* evaluate the lvalue function name *)
+        assert (forall targs tres cc,
+                   eval_expr tge e le_main m_main (reset_name (Tfunction targs tres cc)) (var_ptr ptr_reset)).
+        { intros; eapply eval_Elvalue.
+          - apply eval_Evar_global; eauto.
+          - apply deref_loc_reference; auto.
+        }
+
+        change le_main with (set_opttemp None Vundef le_main).
+        eapply exec_Scall; eauto; simpl; eauto using eval_exprlist.
+        unfold type_of_function.
+        destruct ResetSpec as (-> & -> & -> &?); unfold case_out;
+          rewrite reset_no_output, reset_no_input;
+          erewrite find_class_name; eauto; simpl; auto.
+      Qed.
+
+
+      (*****************************************************************)
+      (** Corollary of exec_body: dostep implies the infinte looping* **)
+      (** execution                                                   **)
+      (** We switch to the small-step semantics since the big-step    **)
+      (** one cannot distinguish between Reacts and Diverges          **)
+      (*****************************************************************)
+
+      Section TraceInf.
+
+        Hypothesis Step_in_spec  : main_step.(m_in) <> [].
+        Hypothesis Step_out_spec : main_step.(m_out) <> [].
+
+        Definition transl_trace (n: nat): traceinf :=
+          traceinf_of_traceinf'
+            (trace_step main_step ins outs Step_in_spec Step_out_spec Hwt_ins Hwt_outs n).
 
         Lemma dostep_loop:
-          forall n meInit le me,
-            wt_mem meInit prog_main c_main ->
-            dostep n me ->
-            execinf_stmt (globalenv tprog) (function_entry2 (globalenv tprog)) e1 le me
-                         (main_loop false main_node m_step)
-                         (traceinf_of_traceinf' (transl_trace n)).
+          forall e n le m,
+            dostep e n m ->
+            execinf_stmt tge (function_entry2 tge) e le m
+                         (main_loop false main_node main_step)
+                         (transl_trace n).
         Proof.
           cofix COINDHYP.
-          intros ????? Hdostep.
-          destruct exec_body with (1:=Hdostep) (le:=le) as (? & ? & ? & ?).
+          intros * Hdostep.
+          destruct exec_body with (1:=Hdostep) (le_n := le) as (? & ? & ? & ?).
           unfold transl_trace, trace_step; rewrite unfold_mk_trace.
           eapply execinf_Sloop_loop with (out1 := Out_normal);
             eauto using out_normal_or_continue, exec_stmt.
         Qed.
 
-        Lemma exec_reset:
-          exists m2,
-            exec_stmt (globalenv tprog) (function_entry2 (globalenv tprog)) e1
-                      le_main m1 (reset_call (c_name c_main)) E0
-                      le_main m2 Out_normal
-            /\ dostep 0 m2.
-        Proof.
-          pose proof methods_corres as MC.
-          destruct dostep_imp as (m2 & Heval & Step); auto.
-          change (eval_funcall tge (function_entry2 tge) m0 (Internal reset_f)
-                               [var_ptr sb] E0 m2 Vundef)
-            with (eval_funcall (globalenv tprog) (function_entry2 (globalenv tprog)) m0 (Internal reset_f)
-                               [var_ptr sb] E0 m2 Vundef) in Heval.
-          pose proof (find_class_name _ _ _ _ Find) as Eq;
-            pose proof (find_method_name _ _ _ Findreset) as Eq';
-            rewrite <-Eq, <-Eq' in *.
-          edestruct MC with (2:=Findreset)
-            as (ptr & f & Get_s & Get_f & Hp_rst & Hr_rst & Hcc_rst
-                & ? & ? & ? & ? & ? & Htr_rst); eauto.
-          rewrite Getreset_s in Get_s; inversion Get_s; subst ptr;
-            rewrite Getreset_f in Get_f; inversion Get_f; subst f.
-          exists m2; split; auto.
-          unfold reset_call.
-          rewrite <-Eq'.
-          change le_main with (set_opttemp None Vundef le_main) at 2.
-          econstructor; simpl; eauto.
-          - eapply eval_Elvalue.
-            + apply eval_Evar_global; eauto.
-              rewrite <-not_Some_is_None.
-              intros (b, t) Hget.
-              subst e1.
-              destruct_list m_step.(m_out).
-              * rewrite PTree.gempty in Hget; discriminate.
-              * rewrite PTree.gempty in Hget; discriminate.
-              *{ rewrite PTree.gso, PTree.gempty in Hget.
-                 - discriminate.
-                 - intro E; apply prefix_injective in E.
-                   + destruct E as [E].
-                     contradict E; apply fun_not_out.
-                   + apply fun_id_valid.
-                   + apply out_valid.
-               }
-            + apply deref_loc_reference; auto.
-          - apply find_method_In in Findreset.
-            do 2 (econstructor; eauto).
-            apply eval_Evar_global; auto.
-            rewrite <-not_Some_is_None.
-            intros (b, t) Hget.
-            subst e1.
-            destruct_list m_step.(m_out).
-            + rewrite PTree.gempty in Hget; discriminate.
-            + rewrite PTree.gempty in Hget; discriminate.
-            + rewrite PTree.gso, PTree.gempty in Hget.
-              * discriminate.
-              *{ intro E; apply (glob_id_not_prefixed self).
-                 - apply self_valid.
-                 - rewrite E; constructor.
-               }
-          - unfold Genv.find_funct. auto.
-          - simpl; unfold type_of_function;
-              rewrite Hp_rst, Hr_rst, Hcc_rst; simpl; repeat f_equal.
-            + rewrite Reset_in_spec; auto.
-              rewrite Reset_out_spec; auto.
-            + rewrite Reset_out_spec; auto.
-        Qed.
-
-        Lemma main_inf:
-          evalinf_funcall (globalenv tprog) (function_entry2 (globalenv tprog)) m0
-                          (Internal main_f) [] (traceinf_of_traceinf' (transl_trace 0)).
-        Proof.
-          pose proof exec_reset as ER. pose proof entry_main as EM.
-          pose proof dostep_loop as DSL.
-          pose proof (find_class_name _ _ _ _ Find) as Eq;
-            pose proof (find_method_name _ _ _ Findreset) as Eq';
-            rewrite <-Eq, <-Eq' in *.
-          destruct Caractmain as (? & ? & ? & ? & ? & Hbody).
-          destruct ER as (? & ? & ?); auto.
-          econstructor; eauto.
-          rewrite <-E0_left_inf, Hbody.
-          eapply execinf_Sseq_1, execinf_Sseq_2; eauto.
-        Qed.
-
         Let after_loop := Kseq (Sreturn (Some cl_zero)) Kstop.
+        Let main_state := Clight.State main_f (main_loop false main_node main_step) after_loop e.
 
         Lemma reactive_loop:
           forall n m le,
-            dostep n m ->
-            Smallstep.forever_reactive (step_fe function_entry2) (globalenv tprog)
-                                       (Clight.State main_f (main_loop false main_node m_step) after_loop e1 le m)
-                                       (traceinf_of_traceinf' (transl_trace n)).
+            dostep e n m ->
+            Forever_reactive (semantics2 tprog) (main_state le m) (transl_trace n).
         Proof.
           unfold transl_trace, trace_step.
           cofix COINDHYP.
           intros * Hdostep'.
           edestruct exec_body with (1:=Hdostep') as (? & ? & Exec_body & ?).
-          eapply exec_stmt_steps in Exec_body.
-          destruct Exec_body as (? & Star_body & Out_body).
+          eapply exec_stmt_steps in Exec_body as (? & Star_body & Out_body).
           unfold main_loop_body in Star_body.
           rewrite unfold_mk_trace.
 
           econstructor; simpl.
-
-          (* eapply Smallstep.star_forever_reactive. *)
-          - eapply Smallstep.star_step.
+          - eapply star_step.
             + eapply step_loop.
-            + eapply Smallstep.star_right with (t2:=E0); auto.
-              *{ eapply Smallstep.star_right with (t2:=E0); auto.
-                 - eapply Star_body.
-                 - inversion_clear Out_body.
+            + eapply star_right with (t2:=E0); auto.
+              * eapply star_right with (t2:=E0); auto.
+                -- eapply Star_body.
+                -- inversion_clear Out_body.
                    apply step_skip_or_continue_loop1; auto.
-               }
               * apply step_skip_loop2.
             + simpl; rewrite 2 E0_right; auto.
           - intro Evts.
             apply app_eq_nil in Evts; destruct Evts.
-            apply (load_events_not_E0 ins (m_in m_step) Step_in_spec Hwt_ins n); auto.
+            apply (load_events_not_E0 ins (m_in main_step) Step_in_spec Hwt_ins n); auto.
           - apply COINDHYP; auto.
         Qed.
 
-        Lemma reacts:
-          program_behaves (semantics2 tprog) (Reacts (traceinf_of_traceinf' (transl_trace 0))).
-        Proof.
-          pose proof entry_main as EM.
-          destruct Caractmain as (Hret & Hcc & Hparams & ? & ? & Hbody).
+        (*****************************************************************)
+        (** We show that the whole program is reactive, with the        **)
+        (** correct infinite trace                                      **)
+        (*****************************************************************)
 
-          destruct exec_reset as (? & Exec_reset & ?).
-          eapply exec_stmt_steps in Exec_reset.
-          destruct Exec_reset as (? & Star_reset & Out_reset).
+        Section Behavior.
 
-          pose proof reactive_loop as RL.
-          pose proof (find_class_name _ _ _ _ Find) as Eq;
-            pose proof (find_method_name _ _ _ Findreset) as Eq';
-            rewrite <-Eq, <-Eq' in *.
-          econstructor.
-          - econstructor; eauto.
-            simpl; unfold type_of_function; auto.
-            rewrite Hparams, Hret, Hcc; auto.
-          -
+          Variable (m0 : mem).
+          Hypothesis Init: Genv.init_mem tprog = Some m0.
+
+          Let prog_state := Clight.Callstate (Internal main_f) [] Kstop m0.
+
+          Lemma initial_state_main:
+            Clight.initial_state tprog prog_state.
+          Proof.
+            intros.
+            edestruct find_main_ptr with (tprog := tprog) (TRANSL := TRANSL) as (?& Find_main &?); eauto.
+            erewrite <- tprog_main_id in Find_main; eauto.
+            econstructor; eauto.
+          Qed.
+
+          Lemma reacts:
+            function_entry2 tge main_f [] m0 e le_main m_main ->
+            program_behaves (semantics2 tprog) (Reacts (transl_trace 0)).
+          Proof.
+            intros.
             econstructor.
-            rewrite <-E0_left_inf.
-            eapply Smallstep.star_forever_reactive.
-            + eapply Smallstep.star_step with (t1:=E0) (t2:=E0); auto.
-              * eapply step_internal_function. eapply EM.
-              *{ eapply Smallstep.star_step with (t1:=E0) (t2:=E0); auto.
-                 - rewrite Hbody.
-                   apply step_seq.
-                 - eapply Smallstep.star_step with (t1:=E0) (t2:=E0); auto.
-                   + apply step_seq.
-                   + eapply Smallstep.star_right with (t1:=E0) (t2:=E0); auto.
-                     * eapply Star_reset.
-                     * inversion_clear Out_reset.
-                       apply step_skip_seq.
-               }
-            + apply RL with (le:=le_main) in H1.
-              unfold after_loop, step_fe in H1. auto.
-        Qed.
+            - apply initial_state_main.
+            - econstructor.
+              destruct exec_reset as (? & Exec_reset & ?).
+              eapply exec_stmt_steps in Exec_reset as (? & Star_reset & Out_reset).
+              rewrite <-E0_left_inf.
+              eapply Smallstep.star_forever_reactive.
+              + eapply star_step with (t1:=E0) (t2:=E0); auto.
+                * eapply step_internal_function; eauto.
+                * eapply star_step with (t1:=E0) (t2:=E0); auto.
+                  -- apply step_seq.
+                  -- eapply star_step with (t1:=E0) (t2:=E0); auto.
+                     ++ apply step_seq.
+                     ++ eapply star_right with (t1:=E0) (t2:=E0); auto.
+                        ** eapply Star_reset.
+                        ** inversion_clear Out_reset.
+                           apply step_skip_seq.
+              + apply reactive_loop; auto.
+          Qed.
 
-      End dostep.
+        End Behavior.
 
-    End Init.
+      End TraceInf.
 
-    Theorem reacts':
-      forall me0 ins outs c_main prog_main m_step m_reset,
-        stmt_call_eval prog mempty (c_name c_main) (m_name m_reset) [] me0 [] ->
-        wt_mem me0 prog_main c_main ->
-        loop_call prog (c_name c_main) step (fun n => map Some (ins n)) (fun n => map Some (outs n)) 0 me0 ->
-        find_class main_node prog = Some (c_main, prog_main) ->
-        find_method reset (c_methods c_main) = Some m_reset ->
-        find_method step (c_methods c_main) = Some m_step ->
-        m_in m_reset = [] ->
-        m_out m_reset = [] ->
-        forall (Step_in_spec: m_in m_step <> []) (Step_out_spec: m_out m_step <> [])
-          (Hwt_in: forall n : nat, wt_vals (ins n) (m_in m_step))
-          (Hwt_out: forall n : nat, wt_vals (outs n) (m_out m_step)),
-          program_behaves (semantics2 tprog)
-                          (Reacts
-                             (traceinf_of_traceinf'
-                                (transl_trace m_step Step_in_spec Step_out_spec ins outs Hwt_in Hwt_out 0))).
-    Proof.
-      intros until m_reset; intros ? ? ? Findmain Findreset Findstep.
-      destruct init_mem as (m0 & sb & Initmem & find_step & Hrep).
-      edestruct (find_main m0 _ Hrep) as
-          (c_main' & prog_main' & m_reset' & m_step' & Findmain' & Findreset' & Findstep' & ? & ? &
-           ? & ? & ? & ? & ? & ? & ? & Hvars & ?  & Hbody & Hmout).
-      rewrite Findmain' in Findmain; inv Findmain; subst.
-      rewrite Findreset' in Findreset; rewrite Findstep' in Findstep; inv Findreset; inv Findstep; subst.
-      edestruct methods_corres with (2:=Findreset')
-        as (? & ? & ? & ? & ? & ? & ? & ? & ? & ? & ? & ?); eauto.
-      edestruct methods_corres with (2:=Findstep')
-        as (? & ? & ? & ? & ? & ? & ? & ? & ? & ? & ? & ?); eauto.
-      intros.
-      case_eq (m_out m_step).
-      - intros Out; rewrite Out in *.
-        eapply reacts with (m_reset:=m_reset) (m_step:=m_step);
-          try rewrite Out; eauto.
-        + repeat split; auto.
-        + rewrite Hvars; econstructor.
-        + erewrite <-sepemp_left, <-sepemp_right; eauto.
-      - intros (x', t') xs Out.
-        destruct xs; rewrite Out in *.
-        + eapply reacts with (m_reset:=m_reset) (m_step:=m_step);
-            try rewrite Out; eauto.
-          * repeat split; auto.
-          * rewrite Hvars; econstructor.
-          * erewrite <-sepemp_left, <-sepemp_right; eauto.
-        + destruct Hmout as (? & ? & ? & ? & ? & ?).
-          eapply reacts; eauto; try rewrite Out; eauto.
-          * repeat split; try rewrite Out; auto.
-          * erewrite sep_swap, <-sepemp_right; eauto.
+    End MainCorrectness.
 
-            Grab Existential Variables.
-            exact empty_co.
-            eauto.
-            exact empty_co.
-            eauto.
-    Qed.
+  End dostep.
 
-    End CORRECTNESS.
+  Lemma out_step_env_empty:
+    out_step_env empty_env.
+  Proof.
+    intros ??? Hin; rewrite PTree.gempty in Hin; discriminate.
+  Qed.
+
+  Lemma out_step_env_set_out_step:
+    forall b t,
+      out_step_env (PTree.set out_step (b, t) empty_env).
+  Proof.
+    intros ????? Hin; rewrite PTree.gsspec in Hin.
+    cases; rewrite PTree.gempty in Hin; discriminate.
+  Qed.
+
+  Program Theorem correctness:
+    forall ins outs me0
+      (WTins        : forall n, wt_vals (ins n) (m_in main_step))
+      (WTouts       : forall n, wt_vals (outs n) (m_out main_step))
+      (Step_in_spec : m_in main_step <> [])
+      (Step_out_spec: m_out main_step <> []),
+      stmt_call_eval prog mempty main_node reset [] me0 [] ->
+      loop_call prog main_node step (fun n => map Some (ins n)) (fun n => map Some (outs n)) 0 me0 ->
+      wt_mem me0 prog_main c_main ->
+      program_behaves (semantics2 tprog) (Reacts (transl_trace ins outs _ _ _ _ 0)).
+  Proof.
+    intros.
+    (* get the reset and step functions *)
+    edestruct methods_corres with (callerid := reset) as (?&?&?&?&?); eauto.
+    edestruct methods_corres with (callerid := step) as (?&?&?&?&?); eauto.
+
+    (* get the self state *)
+    edestruct find_self as (?& FindSelf); eauto.
+
+    (* initialize the memory *)
+    edestruct init_mem as (?&?&?& FindSelf' & Hm); eauto.
+    rewrite FindSelf in FindSelf'; inv FindSelf'.
+
+    (* enter the main function *)
+    pose proof Hm; apply main_entry in Hm.
+
+    cases_eqn E.
+    - destruct Hm as (?& b & co &?&?&?).
+      eapply reacts; eauto.
+      + apply out_step_env_set_out_step.
+      + rewrite E; exists b, co; split; [|split]; auto.
+        apply PTree.gss.
+    - eapply reacts; eauto.
+      * apply out_step_env_empty.
+      * rewrite E; auto.
+  Qed.
 
 End PRESERVATION.
