src/NLustre/NLInterpreter.v
@@ -10,7 +10,7 @@ From Coq Require Import FSets.FMapPositive.
 From Velus Require Import Common.
 From Velus Require Import Environment.
 From Velus Require Import Operators.
-From Velus Require Import Memory.
+From Velus Require Import VelusMemory.
 From Velus Require Import Clocks.
 From Velus Require Import CoreExpr.
 
