src/StcToObc/Stc2ObcTyping.v
@@ -3,7 +3,7 @@ From Velus Require Import Obc.
 
 From Velus Require Import StcToObc.Translation.
 
-From Velus Require Import Memory.
+From Velus Require Import VelusMemory.
 From Velus Require Import Common.
 
 From Coq Require Import List.
